<?xml version="1.0"?>
<rdf:RDF xmlns="https://w3id.org/chint/ontology/"
     xml:base="https://w3id.org/chint/ontology/"
     xmlns:dc="http://purl.org/dc/elements/1.1/"
     xmlns:ldp="http://www.w3.org/ns/ldp#"
     xmlns:owl="http://www.w3.org/2002/07/owl#"
     xmlns:rdf="http://www.w3.org/1999/02/22-rdf-syntax-ns#"
     xmlns:xml="http://www.w3.org/XML/1998/namespace"
     xmlns:xsd="http://www.w3.org/2001/XMLSchema#"
     xmlns:prov="http://www.w3.org/ns/prov#"
     xmlns:rdfs="http://www.w3.org/2000/01/rdf-schema#"
     xmlns:skos="http://www.w3.org/2004/02/skos/core#"
     xmlns:vann="http://purl.org/vocab/vann/"
     xmlns:terms="http://purl.org/dc/terms/"
     xmlns:schema="https://schema.org/">
    <owl:Ontology rdf:about="https://w3id.org/chint/ontology/">
        <owl:imports rdf:resource="http://data.odeuropa.eu/ontology/"/>
        <owl:imports rdf:resource="http://www.cidoc-crm.org/cidoc-crm/"/>
        <owl:imports rdf:resource="http://www.ontologydesignpatterns.org/ont/dul/DUL.owl"/>
        <owl:imports rdf:resource="https://ontology.swissartresearch.net/aaao/"/>
        <owl:imports rdf:resource="https://periodo.github.io/edtf-ontology/edtfo.ttl"/>
        <dc:contributor xml:lang="en">Charles van den Heuvel</dc:contributor>
        <dc:creator>Sofia Baroncini</dc:creator>
        <terms:created>May 2025</terms:created>
        <terms:publisher xml:lang="en">Sofia Baroncini</terms:publisher>
        <terms:title>Cultural Heritage Interactions Ontology </terms:title>
        <vann:preferredNamespacePrefix>chint</vann:preferredNamespacePrefix>
        <rdfs:comment>The Cultural Heritage Interactions Ontology is intended to describe the interactions between material and immaterial cultural heritage (CH) that occur in time. In other words, it relates a CH object with 1) ideas and values that are relevant in the context(s) in which the object is located (i.e., a belief system) 2) the function(s) that such objects acquire in different contexts, 3) the evolution of these features over time, and 4) their interaction with contextual ephemeral events and immaterial cultural heritage practices.</rdfs:comment>
        <owl:versionInfo>0.2</owl:versionInfo>
    </owl:Ontology>
    


    <!-- 
    ///////////////////////////////////////////////////////////////////////////////////////
    //
    // Annotation properties
    //
    ///////////////////////////////////////////////////////////////////////////////////////
     -->

    


    <!-- http://purl.org/dc/elements/1.1/contributor -->

    <owl:AnnotationProperty rdf:about="http://purl.org/dc/elements/1.1/contributor"/>
    


    <!-- http://purl.org/dc/elements/1.1/creator -->

    <owl:AnnotationProperty rdf:about="http://purl.org/dc/elements/1.1/creator"/>
    


    <!-- http://purl.org/dc/terms/created -->

    <owl:AnnotationProperty rdf:about="http://purl.org/dc/terms/created"/>
    


    <!-- http://purl.org/dc/terms/publisher -->

    <owl:AnnotationProperty rdf:about="http://purl.org/dc/terms/publisher"/>
    


    <!-- http://purl.org/dc/terms/title -->

    <owl:AnnotationProperty rdf:about="http://purl.org/dc/terms/title"/>
    


    <!-- http://purl.org/vocab/vann/preferredNamespacePrefix -->

    <owl:AnnotationProperty rdf:about="http://purl.org/vocab/vann/preferredNamespacePrefix"/>
    


    <!-- http://www.w3.org/2002/07/owl#cardinality -->

    <owl:AnnotationProperty rdf:about="http://www.w3.org/2002/07/owl#cardinality"/>
    


    <!-- http://www.w3.org/2002/07/owl#maxCardinality -->

    <owl:AnnotationProperty rdf:about="http://www.w3.org/2002/07/owl#maxCardinality"/>
    


    <!-- http://www.w3.org/2002/07/owl#minCardinality -->

    <owl:AnnotationProperty rdf:about="http://www.w3.org/2002/07/owl#minCardinality"/>
    


    <!-- http://www.w3.org/2004/02/skos/core#definition -->

    <owl:AnnotationProperty rdf:about="http://www.w3.org/2004/02/skos/core#definition"/>
    


    <!-- http://www.w3.org/2004/02/skos/core#example -->

    <owl:AnnotationProperty rdf:about="http://www.w3.org/2004/02/skos/core#example"/>
    


    <!-- http://www.w3.org/2004/02/skos/core#notation -->

    <owl:AnnotationProperty rdf:about="http://www.w3.org/2004/02/skos/core#notation"/>
    


    <!-- 
    ///////////////////////////////////////////////////////////////////////////////////////
    //
    // Object Properties
    //
    ///////////////////////////////////////////////////////////////////////////////////////
     -->

    


    <!-- http://data.odeuropa.eu/ontology/F1_generated -->

    <owl:ObjectProperty rdf:about="http://data.odeuropa.eu/ontology/F1_generated">
        <rdfs:subPropertyOf rdf:resource="http://erlangen-crm.org/current/P92_brought_into_existence"/>
        <rdf:type rdf:resource="http://www.w3.org/2002/07/owl#AsymmetricProperty"/>
        <rdfs:domain rdf:resource="http://data.odeuropa.eu/ontology/L2_Stimulus_Generation"/>
        <rdfs:range rdf:resource="http://data.odeuropa.eu/ontology/L1_Sensory_Stimulus"/>
        <rdfs:comment xml:lang="en">This property associates an instance of L2 Stimulus Generation with the L1 Sensory Stimulus which was created by the event.</rdfs:comment>
        <owl:cardinality rdf:datatype="http://www.w3.org/2001/XMLSchema#nonNegativeInteger">1</owl:cardinality>
    </owl:ObjectProperty>
    


    <!-- http://data.odeuropa.eu/ontology/F2_perceived -->

    <owl:ObjectProperty rdf:about="http://data.odeuropa.eu/ontology/F2_perceived">
        <rdfs:subPropertyOf rdf:resource="http://www.ics.forth.gr/isl/CRMsci/O8_observed"/>
        <rdf:type rdf:resource="http://www.w3.org/2002/07/owl#AsymmetricProperty"/>
        <rdfs:domain rdf:resource="http://data.odeuropa.eu/ontology/L3_Sensory_Experience"/>
        <rdfs:range rdf:resource="http://data.odeuropa.eu/ontology/L1_Sensory_Stimulus"/>
        <rdfs:comment xml:lang="en">This property associates an instance of L3 Sensory Experience with the L1 Sensory Stimulus which was experienced.</rdfs:comment>
        <owl:cardinality rdf:datatype="http://www.w3.org/2001/XMLSchema#nonNegativeInteger">1</owl:cardinality>
    </owl:ObjectProperty>
    


    <!-- http://data.odeuropa.eu/ontology/F6_evoked -->

    <owl:ObjectProperty rdf:about="http://data.odeuropa.eu/ontology/F6_evoked">
        <rdfs:subPropertyOf rdf:resource="http://erlangen-crm.org/current/P15_was_influenced_by"/>
        <rdfs:domain rdf:resource="http://data.odeuropa.eu/ontology/L3_Sensory_Experience"/>
        <rdfs:comment xml:lang="en">This property associates an instance of L3 Sensory Experience with a (material or conceptual) entity which is evoked during the experience itself. This includes memories of people or situations, comparison to similar stimuli, references, etc.</rdfs:comment>
    </owl:ObjectProperty>
    


    <!-- http://erlangen-crm.org/current/P15_was_influenced_by -->

    <owl:ObjectProperty rdf:about="http://erlangen-crm.org/current/P15_was_influenced_by"/>
    


    <!-- http://erlangen-crm.org/current/P92_brought_into_existence -->

    <owl:ObjectProperty rdf:about="http://erlangen-crm.org/current/P92_brought_into_existence"/>
    


    <!-- http://www.cidoc-crm.org/cidoc-crm/P10_falls_within -->

    <owl:ObjectProperty rdf:about="http://www.cidoc-crm.org/cidoc-crm/P10_falls_within">
        <rdfs:subPropertyOf rdf:resource="http://www.cidoc-crm.org/cidoc-crm/P132_spatiotemporally_overlaps_with"/>
        <owl:inverseOf rdf:resource="http://www.cidoc-crm.org/cidoc-crm/P10i_contains"/>
        <rdfs:domain rdf:resource="http://www.cidoc-crm.org/cidoc-crm/E92_Spacetime_Volume"/>
        <rdfs:range rdf:resource="http://www.cidoc-crm.org/cidoc-crm/E92_Spacetime_Volume"/>
        <rdfs:comment xml:lang="en">This property associates an instance of E92 Spacetime Volume with another instance of E92 Spacetime Volume that falls within the latter. In other words, all points in the former are also points in the latter.
This property is transitive and reflexive.</rdfs:comment>
        <rdfs:label xml:lang="en">falls within</rdfs:label>
    </owl:ObjectProperty>
    


    <!-- http://www.cidoc-crm.org/cidoc-crm/P10i_contains -->

    <owl:ObjectProperty rdf:about="http://www.cidoc-crm.org/cidoc-crm/P10i_contains">
        <rdfs:subPropertyOf rdf:resource="http://www.cidoc-crm.org/cidoc-crm/P132_spatiotemporally_overlaps_with"/>
        <rdfs:domain rdf:resource="http://www.cidoc-crm.org/cidoc-crm/E92_Spacetime_Volume"/>
        <rdfs:range rdf:resource="http://www.cidoc-crm.org/cidoc-crm/E92_Spacetime_Volume"/>
        <rdfs:label xml:lang="en">contains</rdfs:label>
    </owl:ObjectProperty>
    


    <!-- http://www.cidoc-crm.org/cidoc-crm/P110_augmented -->

    <owl:ObjectProperty rdf:about="http://www.cidoc-crm.org/cidoc-crm/P110_augmented">
        <rdfs:subPropertyOf rdf:resource="http://www.cidoc-crm.org/cidoc-crm/P31_has_modified"/>
        <rdfs:domain rdf:resource="http://www.cidoc-crm.org/cidoc-crm/E79_Part_Addition"/>
        <rdfs:range rdf:resource="http://www.cidoc-crm.org/cidoc-crm/E18_Physical_Thing"/>
        <rdfs:comment xml:lang="en">This property identifies the instance of E24 Physical Human-Made Thing that is added to (augmented) in an instance of E79 Part Addition.Although an instance of E79 Part Addition event normally concerns only one instance of E24 Physical Human-Made Thing, it is possible to imagine circumstances under which more than one item might be added to (augmented). For example, the artist Jackson Pollock trailing paint onto multiple canvasses.</rdfs:comment>
        <rdfs:label xml:lang="en">augmented</rdfs:label>
        <skos:notation>P110</skos:notation>
    </owl:ObjectProperty>
    


    <!-- http://www.cidoc-crm.org/cidoc-crm/P111_added -->

    <owl:ObjectProperty rdf:about="http://www.cidoc-crm.org/cidoc-crm/P111_added">
        <rdfs:subPropertyOf rdf:resource="http://www.cidoc-crm.org/cidoc-crm/P16_used_specific_object"/>
        <rdfs:domain rdf:resource="http://www.cidoc-crm.org/cidoc-crm/E79_Part_Addition"/>
        <rdfs:range rdf:resource="http://www.cidoc-crm.org/cidoc-crm/E18_Physical_Thing"/>
        <rdfs:comment xml:lang="en">This property identifies the instance of E18 Physical Thing that is added during an instance of E79 Part Addition activity.</rdfs:comment>
        <rdfs:label xml:lang="en">added</rdfs:label>
        <skos:notation>P111</skos:notation>
    </owl:ObjectProperty>
    


    <!-- http://www.cidoc-crm.org/cidoc-crm/P112_diminished -->

    <owl:ObjectProperty rdf:about="http://www.cidoc-crm.org/cidoc-crm/P112_diminished">
        <rdfs:subPropertyOf rdf:resource="http://www.cidoc-crm.org/cidoc-crm/P31_has_modified"/>
        <rdfs:domain rdf:resource="http://www.cidoc-crm.org/cidoc-crm/E80_Part_Removal"/>
        <rdfs:range rdf:resource="http://www.cidoc-crm.org/cidoc-crm/E18_Physical_Thing"/>
        <rdfs:comment xml:lang="en">This property identifies the instance of E18 Physical Thing that was diminished by an instance of E80 Part Removal.Although an instance of E80 Part removal activity normally concerns only one instance of E18 Physical Thing, it is possible to imagine circumstances under which more than one item might be diminished by a single instance of E80 Part Removal activity. </rdfs:comment>
        <rdfs:label xml:lang="en">diminished</rdfs:label>
        <skos:notation>P112</skos:notation>
    </owl:ObjectProperty>
    


    <!-- http://www.cidoc-crm.org/cidoc-crm/P113_removed -->

    <owl:ObjectProperty rdf:about="http://www.cidoc-crm.org/cidoc-crm/P113_removed">
        <rdfs:subPropertyOf rdf:resource="http://www.cidoc-crm.org/cidoc-crm/P12_occurred_in_the_presence_of"/>
        <rdfs:domain rdf:resource="http://www.cidoc-crm.org/cidoc-crm/E80_Part_Removal"/>
        <rdfs:range rdf:resource="http://www.cidoc-crm.org/cidoc-crm/E18_Physical_Thing"/>
        <rdfs:comment xml:lang="en">This property identifies the instance of E18 Physical Thing that is removed during an instance of E80 Part Removal activity.</rdfs:comment>
        <rdfs:label xml:lang="en">removed</rdfs:label>
        <skos:notation>P113</skos:notation>
    </owl:ObjectProperty>
    


    <!-- http://www.cidoc-crm.org/cidoc-crm/P11_had_participant -->

    <owl:ObjectProperty rdf:about="http://www.cidoc-crm.org/cidoc-crm/P11_had_participant">
        <rdfs:subPropertyOf rdf:resource="http://www.cidoc-crm.org/cidoc-crm/P12_occurred_in_the_presence_of"/>
        <rdfs:domain rdf:resource="http://www.cidoc-crm.org/cidoc-crm/E5_Event"/>
        <rdfs:range rdf:resource="http://www.cidoc-crm.org/cidoc-crm/E39_Actor"/>
        <rdfs:comment xml:lang="en">This property describes the active or passive participation of instances of E39 Actors in an instance of E5 Event. It documents known events in which an instance of E39 Actor has participated during the course of that actor’s life or history. The instances of E53 Place and E52 Time-Span where and when these events happened provide us with constraints about the presence of the related instances of E39 Actor in the past. Collective actors, i.e., instances of E74 Group, may physically participate in events via their representing instances of E21 Persons only. The participation of multiple actors in an event is most likely an indication of their acquaintance and interaction.The property implies that the actor was involved in the event but does not imply any causal relationship. For instance, someone having been portrayed can be said to have participated in the creation of the portrait.</rdfs:comment>
        <rdfs:label xml:lang="en">had participant</rdfs:label>
        <skos:notation>P11</skos:notation>
    </owl:ObjectProperty>
    


    <!-- http://www.cidoc-crm.org/cidoc-crm/P123_resulted_in -->

    <owl:ObjectProperty rdf:about="http://www.cidoc-crm.org/cidoc-crm/P123_resulted_in">
        <rdfs:subPropertyOf rdf:resource="http://www.cidoc-crm.org/cidoc-crm/P92_brought_into_existence"/>
        <rdfs:range rdf:resource="http://www.cidoc-crm.org/cidoc-crm/E18_Physical_Thing"/>
        <rdfs:comment xml:lang="en">This property identifies the instance or instances of E18 Physical Thing that are the result of an instance of E81 Transformation. New items replace the transformed item or items, which cease to exist as units of documentation. The physical continuity between the old and the new is expressed by the links to the common instance of E81 Transformation.</rdfs:comment>
        <rdfs:label xml:lang="en">resulted in</rdfs:label>
        <skos:notation>P123</skos:notation>
    </owl:ObjectProperty>
    


    <!-- http://www.cidoc-crm.org/cidoc-crm/P124_transformed -->

    <owl:ObjectProperty rdf:about="http://www.cidoc-crm.org/cidoc-crm/P124_transformed">
        <rdfs:subPropertyOf rdf:resource="http://www.cidoc-crm.org/cidoc-crm/P93_took_out_of_existence"/>
        <rdfs:range rdf:resource="http://www.cidoc-crm.org/cidoc-crm/E18_Physical_Thing"/>
        <rdfs:comment xml:lang="en">This property identifies the instance or instances E18 Physical Thing that have ceased to exist due to an instance of E81 Transformation.The item that has ceased to exist and was replaced by the result of the Transformation. The continuity between both items, the new and the old, is expressed by the links to the common instance of E81 Transformation.</rdfs:comment>
        <rdfs:label xml:lang="en">transformed</rdfs:label>
        <skos:notation>P124</skos:notation>
    </owl:ObjectProperty>
    


    <!-- http://www.cidoc-crm.org/cidoc-crm/P128_carries -->

    <owl:ObjectProperty rdf:about="http://www.cidoc-crm.org/cidoc-crm/P128_carries"/>
    


    <!-- http://www.cidoc-crm.org/cidoc-crm/P12_occurred_in_the_presence_of -->

    <owl:ObjectProperty rdf:about="http://www.cidoc-crm.org/cidoc-crm/P12_occurred_in_the_presence_of">
        <rdfs:domain rdf:resource="http://www.cidoc-crm.org/cidoc-crm/E5_Event"/>
        <rdfs:range rdf:resource="http://www.cidoc-crm.org/cidoc-crm/E77_Persistent_Item"/>
        <rdfs:comment xml:lang="en">This property describes the active or passive presence of an E77 Persistent Item in an instance of E5 Event without implying any specific role. It documents known events in which an instance of E77 Persistent Item was present during the course of its life or history. For example, an object may be the desk, now in a museum, on which a treaty was signed. The instance of E53 Place and the instance of E52 Time-Span where and when these events happened provide us with constraints about the presence of the related instance E77 Persistent Item in the past. Instances of E90 Symbolic Object, in particular information objects, are physically present in events via at least one of the instances of E18 Physical Thing carrying them. Note, that the human mind can be such a carrier. A precondition for a transfer of information to a person or another new physical carrier is the presence of the respective information object and this person or physical thing in one event.</rdfs:comment>
        <rdfs:label xml:lang="en">occurred in the presence of</rdfs:label>
        <skos:notation>P12</skos:notation>
    </owl:ObjectProperty>
    


    <!-- http://www.cidoc-crm.org/cidoc-crm/P132_spatiotemporally_overlaps_with -->

    <owl:ObjectProperty rdf:about="http://www.cidoc-crm.org/cidoc-crm/P132_spatiotemporally_overlaps_with">
        <rdfs:domain rdf:resource="http://www.cidoc-crm.org/cidoc-crm/E92_Spacetime_Volume"/>
        <rdfs:range rdf:resource="http://www.cidoc-crm.org/cidoc-crm/E92_Spacetime_Volume"/>
        <rdfs:comment xml:lang="en">This symmetric property associates two instances of E92 Spacetime Volume that have some of their extents in common. If only the fuzzy boundaries of the instances of E92 Spacetime Volume overlap, this property cannot be determined from observation alone and therefore should not be applied. However, there may be other forms of justification that the two instances of E92 Spacetime Volume must have some of their extents in common regardless of where and when precisely.
If this property holds for two instances of E92 Spacetime Volume then it cannot be the case that P133 is spatiotemporally separated from also holds for the same two instances. Furthermore, there are cases where neither P132 spatiotemporally overlaps with nor P133 is spatiotemporally separated from holds between two instances of E92 Spacetime Volume. This would occur where only an overlap of the fuzzy boundaries of the two instances of E92 Spacetime Volume occurs and no other evidence is available.
This property is not transitive. This property is symmetric. This property is reflexive.</rdfs:comment>
        <rdfs:label xml:lang="en">spatiotemporally overlaps with</rdfs:label>
    </owl:ObjectProperty>
    


    <!-- http://www.cidoc-crm.org/cidoc-crm/P133_is_spatiotemporally_separated_from -->

    <owl:ObjectProperty rdf:about="http://www.cidoc-crm.org/cidoc-crm/P133_is_spatiotemporally_separated_from">
        <rdfs:domain rdf:resource="http://www.cidoc-crm.org/cidoc-crm/E92_Spacetime_Volume"/>
        <rdfs:range rdf:resource="http://www.cidoc-crm.org/cidoc-crm/E92_Spacetime_Volume"/>
        <rdfs:comment xml:lang="en">This symmetric property associates two instances of E92 Spacetime Volume that have no extents in common. If only the fuzzy boundaries of the instances of E92 Spacetime Volume overlap, this property cannot be determined from observation alone and therefore should not be applied. However, there may be other forms of justification that the two instances of E92 Spacetime Volume must not have any of their extents in common regardless of where and when precisely.
If this property holds for two instances of E92 Spacetime Volume then it cannot be the case that P132 spatiotemporally overlaps with also holds for the same two instances. Furthermore, there are cases where neither P132 spatiotemporally overlaps with nor P133 is spatiotemporally separated from holds between two instances of E92 Spacetime Volume. This would occur where only an overlap of the fuzzy boundaries of the two instances of E92 Spacetime Volume occurs and no other evidence is available.
This property is not transitive. This property is symmetric. This property is irreflexive.</rdfs:comment>
        <rdfs:label xml:lang="en">is spatiotemporally separated from</rdfs:label>
    </owl:ObjectProperty>
    


    <!-- http://www.cidoc-crm.org/cidoc-crm/P160_has_temporal_projection -->

    <owl:ObjectProperty rdf:about="http://www.cidoc-crm.org/cidoc-crm/P160_has_temporal_projection">
        <owl:inverseOf rdf:resource="http://www.cidoc-crm.org/cidoc-crm/P160i_is_temporal_projection_of"/>
        <rdfs:domain rdf:resource="http://www.cidoc-crm.org/cidoc-crm/E92_Spacetime_Volume"/>
        <rdfs:range rdf:resource="http://www.cidoc-crm.org/cidoc-crm/E52_Time-Span"/>
        <rdfs:comment xml:lang="en">This property describes the temporal projection of an instance of E92 Spacetime Volume. The property P4 has time-span is the same as P160 has temporal projection if it is used to document an instance of E4 Period or any subclass of it.</rdfs:comment>
        <rdfs:label xml:lang="en">has temporal projection</rdfs:label>
    </owl:ObjectProperty>
    


    <!-- http://www.cidoc-crm.org/cidoc-crm/P160i_is_temporal_projection_of -->

    <owl:ObjectProperty rdf:about="http://www.cidoc-crm.org/cidoc-crm/P160i_is_temporal_projection_of"/>
    


    <!-- http://www.cidoc-crm.org/cidoc-crm/P161_has_spatial_projection -->

    <owl:ObjectProperty rdf:about="http://www.cidoc-crm.org/cidoc-crm/P161_has_spatial_projection">
        <owl:inverseOf rdf:resource="http://www.cidoc-crm.org/cidoc-crm/P161i_is_spatial_projection_of"/>
        <rdfs:domain rdf:resource="http://www.cidoc-crm.org/cidoc-crm/E92_Spacetime_Volume"/>
        <rdfs:range rdf:resource="http://www.cidoc-crm.org/cidoc-crm/E53_Place"/>
        <rdfs:comment xml:lang="en">This property associates an instance of E92 Spacetime Volume with an instance of E53 Place that is the result of the spatial projection of the instance of the E92 Spacetime Volume on a reference space.
In general, there can be more than one useful reference space (for reference space see P156 occupies and P157 is at rest relative to) to describe the spatial projection of a spacetime volume, for example, in describing a sea battle, the difference between the battle ship and the seafloor as reference spaces. Thus, it can be seen that the projection is not unique.
The spatial projection is the actual spatial coverage of a spacetime volume, which normally has fuzzy boundaries except for instances of E92 Spacetime Volume which are geometrically defined in the same reference system as the range of this property and are an exception to this and do not have fuzzy boundaries. Modelling explicitly fuzzy spatial projections serves therefore as a common topological reference of different spatial approximations rather than absolute geometric determination, for instance for relating outer or inner spatial boundaries for the respective spacetime volumes.
The spatial projection is unique with respect to the reference system. For instance, there is exactly one spatial projection of Lord Nelson’s dying relative to the ship HMS Victory, i.e. the location of his body relative to the ship HMS Victory at the time of his death.
In case the domain of an instance of P161 has spatial projection is an instance of E4 Period, the spatial projection describes all areas that period was ever present at, for instance, the Roman Empire.
This property is part of the fully developed path from E18 Physical Thing through P196 defines, E92 Spacetime Volume, P161 has spatial projection to E53 Place, which in turn is implied by P156 occupies (is occupied by).</rdfs:comment>
        <rdfs:label xml:lang="en">has spatial projection</rdfs:label>
    </owl:ObjectProperty>
    


    <!-- http://www.cidoc-crm.org/cidoc-crm/P161i_is_spatial_projection_of -->

    <owl:ObjectProperty rdf:about="http://www.cidoc-crm.org/cidoc-crm/P161i_is_spatial_projection_of"/>
    


    <!-- http://www.cidoc-crm.org/cidoc-crm/P16_used_specific_object -->

    <owl:ObjectProperty rdf:about="http://www.cidoc-crm.org/cidoc-crm/P16_used_specific_object"/>
    


    <!-- http://www.cidoc-crm.org/cidoc-crm/P2_has_type -->

    <owl:ObjectProperty rdf:about="http://www.cidoc-crm.org/cidoc-crm/P2_has_type">
        <rdfs:domain rdf:resource="http://www.cidoc-crm.org/cidoc-crm/E1_CRM_Entity"/>
        <rdfs:range rdf:resource="http://www.cidoc-crm.org/cidoc-crm/E55_Type"/>
        <rdfs:comment xml:lang="en">This property allows sub typing of CIDOC CRM entities –a form of specialisation – through the use of a terminological hierarchy, or thesaurus. The CIDOC CRM is intended to focus on the high-level entities and relationships needed to describe data structures. Consequently, it does not specialise entities any further than is required for this immediate purpose. However, entities in the isA hierarchy of the CIDOC CRM may by specialised into any number of sub entities, which can be defined in the E55 Type hierarchy. E41 Appellation, for example, may be specialised into “e-mail address”, “telephone number”, “post office box”, “URL” etc. none of which figures explicitly in the CIDOC CRM hierarchy. A comprehensive explanation about refining CIDOC CRM concepts by E55 Type is given in the section “About Types” in the section on “Specific Modelling Constructs” of this document.This property is a shortcut for the path from E1 CRM Entity through P41i was classified by, E17 Type Assignment, P42 assigned to E55 Type.</rdfs:comment>
        <rdfs:label xml:lang="en">has type</rdfs:label>
        <skos:notation>P2</skos:notation>
    </owl:ObjectProperty>
    


    <!-- http://www.cidoc-crm.org/cidoc-crm/P31_has_modified -->

    <owl:ObjectProperty rdf:about="http://www.cidoc-crm.org/cidoc-crm/P31_has_modified"/>
    


    <!-- http://www.cidoc-crm.org/cidoc-crm/P3_has_note -->

    <owl:ObjectProperty rdf:about="http://www.cidoc-crm.org/cidoc-crm/P3_has_note"/>
    


    <!-- http://www.cidoc-crm.org/cidoc-crm/P45_consists_of -->

    <owl:ObjectProperty rdf:about="http://www.cidoc-crm.org/cidoc-crm/P45_consists_of">
        <rdfs:domain rdf:resource="http://www.cidoc-crm.org/cidoc-crm/E18_Physical_Thing"/>
        <rdfs:range rdf:resource="http://www.cidoc-crm.org/cidoc-crm/E57_Material"/>
        <rdfs:comment xml:lang="en">This property identifies the instances of E57 Materials of which an instance of E18 Physical Thing is composed.All physical things consist of physical materials. P45 consists of (is incorporated in) allows the different materials to be recorded. P45 consists of (is incorporated in) refers here to observed material as opposed to the consumed raw material.A material, such as a theoretical alloy, may not have any physical instances.</rdfs:comment>
        <rdfs:label xml:lang="en">consists of</rdfs:label>
        <skos:notation>P45</skos:notation>
    </owl:ObjectProperty>
    


    <!-- http://www.cidoc-crm.org/cidoc-crm/P4_has_time-span -->

    <owl:ObjectProperty rdf:about="http://www.cidoc-crm.org/cidoc-crm/P4_has_time-span">
        <rdfs:domain rdf:resource="http://www.cidoc-crm.org/cidoc-crm/E2_Temporal_Entity"/>
        <rdfs:range rdf:resource="http://www.cidoc-crm.org/cidoc-crm/E52_Time-Span"/>
        <rdfs:comment xml:lang="en">This property associates an instance of E2 Temporal Entity with the instance of E52 Time-Span during which it was on-going. The associated instance of E52 Time-Span is understood as the real time-span during which the phenomena making up the temporal entity instance were active. More than one instance of E2 Temporal Entity may share a common instance of E52 Time-Span only if they come into being and end being due to identical declarations or events.</rdfs:comment>
        <rdfs:label xml:lang="en">has time-span</rdfs:label>
        <skos:notation>P4</skos:notation>
    </owl:ObjectProperty>
    


    <!-- http://www.cidoc-crm.org/cidoc-crm/P65_shows_visual_item -->

    <owl:ObjectProperty rdf:about="http://www.cidoc-crm.org/cidoc-crm/P65_shows_visual_item">
        <rdfs:subPropertyOf rdf:resource="http://www.cidoc-crm.org/cidoc-crm/P128_carries"/>
        <rdfs:domain rdf:resource="http://www.cidoc-crm.org/cidoc-crm/E24_Physical_Human-Made_Thing"/>
        <rdfs:range rdf:resource="http://www.cidoc-crm.org/cidoc-crm/E36_Visual_Item"/>
        <rdfs:comment xml:lang="en">This property documents an instance of E36 Visual Item shown by an instance of E24 Physical Human-Made Thing.This property is similar to P62 depicts (is depicted by) in that it associates an instance of E24 Physical Human-Made Thing with a visual representation. However, P65 shows visual item (is shown by) differs from the P62 depicts (is depicted by) property in that it makes no claims about what the instance of E36 Visual Item is deemed to represent. An instance of E36 Visual Item identifies a recognisable image or visual symbol, regardless of what this image may or may not represent.For example, all recent British coins bear a portrait of Queen Elizabeth II, a fact that is correctly documented using P62 depicts (is depicted by). Different portraits have been used at different periods, however. P65 shows visual item (is shown by) can be used to refer to a particular portrait.P65 shows visual item (is shown by) may also be used for Visual Items such as signs, marks and symbols, for example the &apos;&apos;Maltese Cross&apos;&apos; or the &apos;&apos;copyright symbol’ that have no particular representational content. This property is part of the fully developed path E24 Physical Human-Made Thing, P65 shows visual item, E36 Visual Item, P138 represents to E1 CRM Entity which is shortcut by, P62 depicts (is depicted by).</rdfs:comment>
        <rdfs:label xml:lang="en">shows visual item</rdfs:label>
        <skos:notation>P65</skos:notation>
    </owl:ObjectProperty>
    


    <!-- http://www.cidoc-crm.org/cidoc-crm/P79_beginning_is_qualified_by -->

    <owl:ObjectProperty rdf:about="http://www.cidoc-crm.org/cidoc-crm/P79_beginning_is_qualified_by">
        <rdfs:subPropertyOf rdf:resource="http://www.cidoc-crm.org/cidoc-crm/P3_has_note"/>
        <rdfs:domain rdf:resource="http://www.cidoc-crm.org/cidoc-crm/E52_Time-Span"/>
        <rdfs:comment xml:lang="en">This property associates an instance of E52 Time-Span with a note detailing the scholarly or scientific opinions and justifications about the certainty, precision, sources etc. of its beginning. Such notes may also be used to elaborate arguments about constraints or to give explanations of alternatives.</rdfs:comment>
        <rdfs:label xml:lang="en">beginning is qualified by</rdfs:label>
        <skos:notation>P79</skos:notation>
    </owl:ObjectProperty>
    


    <!-- http://www.cidoc-crm.org/cidoc-crm/P80_end_is_qualified_by -->

    <owl:ObjectProperty rdf:about="http://www.cidoc-crm.org/cidoc-crm/P80_end_is_qualified_by">
        <rdfs:subPropertyOf rdf:resource="http://www.cidoc-crm.org/cidoc-crm/P3_has_note"/>
        <rdfs:domain rdf:resource="http://www.cidoc-crm.org/cidoc-crm/E52_Time-Span"/>
        <rdfs:comment xml:lang="en">This property associates an instance of E52 Time-Span with a note detailing the scholarly or scientific opinions and justifications about the end of this time-span concerning certainty, precision, sources etc. This property may also be used to describe arguments constraining possible dates and to distinguish reasons for alternative dates.</rdfs:comment>
        <rdfs:label xml:lang="en">end is qualified by</rdfs:label>
        <skos:notation>P80</skos:notation>
    </owl:ObjectProperty>
    


    <!-- http://www.cidoc-crm.org/cidoc-crm/P81_ongoing_throughout -->

    <owl:ObjectProperty rdf:about="http://www.cidoc-crm.org/cidoc-crm/P81_ongoing_throughout">
        <rdfs:domain rdf:resource="http://www.cidoc-crm.org/cidoc-crm/E52_Time-Span"/>
        <rdfs:comment xml:lang="en">This property associates an instance of E52 Time-Span with an instance of E61 Time Primitive specifying a minimum period of time covered by it. Since Time-Spans may not have precisely known temporal extents, the CIDOC CRM supports statements about the minimum and maximum temporal extents of Time-Spans. This property allows a Time-Span’s minimum temporal extent (i.e., its inner boundary) to be assigned an E61 Time Primitive value. Time Primitives are treated by the CIDOC CRM as application or system specific date intervals, and are not further analysed. If different sources of evidence justify different minimum extents without contradicting each other, the smallest interval including all these extents will be the best estimate. This should be taken into account for information integration.</rdfs:comment>
        <rdfs:label xml:lang="en">ongoing throughout</rdfs:label>
        <skos:notation>P81</skos:notation>
    </owl:ObjectProperty>
    


    <!-- http://www.cidoc-crm.org/cidoc-crm/P82_at_some_time_within -->

    <owl:ObjectProperty rdf:about="http://www.cidoc-crm.org/cidoc-crm/P82_at_some_time_within">
        <rdfs:domain rdf:resource="http://www.cidoc-crm.org/cidoc-crm/E52_Time-Span"/>
        <rdfs:comment xml:lang="en">This property describes the maximum period of time within which an E52 Time-Span falls. Since Time-Spans may not have precisely known temporal extents, the CIDOC CRM supports statements about the minimum and maximum temporal extents of Time-Spans. This property allows a Time-Span’s maximum temporal extent (i.e., its outer boundary) to be assigned an E61 Time Primitive value. Time Primitives are treated by the CIDOC CRM as application or system specific date intervals, and are not further analysed. If different sources of evidence justify different maximum extents without contradicting each other, the resulting intersection of all these extents will be the best estimate. This should be taken into account for information integration.</rdfs:comment>
        <rdfs:label xml:lang="en">at some time within</rdfs:label>
        <skos:notation>P82</skos:notation>
    </owl:ObjectProperty>
    


    <!-- http://www.cidoc-crm.org/cidoc-crm/P92_brought_into_existence -->

    <owl:ObjectProperty rdf:about="http://www.cidoc-crm.org/cidoc-crm/P92_brought_into_existence"/>
    


    <!-- http://www.cidoc-crm.org/cidoc-crm/P93_took_out_of_existence -->

    <owl:ObjectProperty rdf:about="http://www.cidoc-crm.org/cidoc-crm/P93_took_out_of_existence"/>
    


    <!-- http://www.ics.forth.gr/isl/CRMsci/O8_observed -->

    <owl:ObjectProperty rdf:about="http://www.ics.forth.gr/isl/CRMsci/O8_observed"/>
    


    <!-- http://www.ontologydesignpatterns.org/ont/dul/DUL.owl#associatedWith -->

    <owl:ObjectProperty rdf:about="http://www.ontologydesignpatterns.org/ont/dul/DUL.owl#associatedWith"/>
    


    <!-- http://www.ontologydesignpatterns.org/ont/dul/DUL.owl#classifies -->

    <owl:ObjectProperty rdf:about="http://www.ontologydesignpatterns.org/ont/dul/DUL.owl#classifies"/>
    


    <!-- http://www.ontologydesignpatterns.org/ont/dul/DUL.owl#follows -->

    <owl:ObjectProperty rdf:about="http://www.ontologydesignpatterns.org/ont/dul/DUL.owl#follows">
        <owl:inverseOf rdf:resource="http://www.ontologydesignpatterns.org/ont/dul/DUL.owl#precedes"/>
    </owl:ObjectProperty>
    


    <!-- http://www.ontologydesignpatterns.org/ont/dul/DUL.owl#hasMember -->

    <owl:ObjectProperty rdf:about="http://www.ontologydesignpatterns.org/ont/dul/DUL.owl#hasMember">
        <rdfs:subPropertyOf rdf:resource="http://www.ontologydesignpatterns.org/ont/dul/DUL.owl#associatedWith"/>
        <owl:inverseOf rdf:resource="http://www.ontologydesignpatterns.org/ont/dul/DUL.owl#isMemberOf"/>
        <rdfs:domain rdf:resource="http://www.ontologydesignpatterns.org/ont/dul/DUL.owl#Collection"/>
        <rdfs:range rdf:resource="http://www.ontologydesignpatterns.org/ont/dul/DUL.owl#Entity"/>
        <owl:propertyChainAxiom rdf:parseType="Collection">
            <rdf:Description rdf:about="https://w3id.org/chint/ontology/hasMemberEvent"/>
        </owl:propertyChainAxiom>
        <rdfs:comment>A relation between collections and entities, e.g. &apos;my collection of saxophones includes an old Adolphe Sax original alto&apos; (i.e. my collection has member an Adolphe Sax alto).</rdfs:comment>
        <rdfs:isDefinedBy rdf:resource="http://www.ontologydesignpatterns.org/ont/dul/DUL.owl"/>
        <rdfs:label xml:lang="en">has member</rdfs:label>
    </owl:ObjectProperty>
    


    <!-- http://www.ontologydesignpatterns.org/ont/dul/DUL.owl#hasParticipant -->

    <owl:ObjectProperty rdf:about="http://www.ontologydesignpatterns.org/ont/dul/DUL.owl#hasParticipant">
        <rdfs:subPropertyOf rdf:resource="http://www.ontologydesignpatterns.org/ont/dul/DUL.owl#associatedWith"/>
        <rdfs:range rdf:resource="http://www.ontologydesignpatterns.org/ont/dul/DUL.owl#Object"/>
        <rdfs:comment>A relation between an object and a process, e.g. &apos;John took part in the discussion&apos;, &apos;a large mass of snow fell during the avalanche&apos;, or &apos;a cook, some sugar, flour, etc. are all present in the cooking of a cake&apos;.</rdfs:comment>
        <rdfs:isDefinedBy rdf:resource="http://www.ontologydesignpatterns.org/ont/dul/DUL.owl"/>
        <rdfs:label xml:lang="en">has participant</rdfs:label>
    </owl:ObjectProperty>
    


    <!-- http://www.ontologydesignpatterns.org/ont/dul/DUL.owl#hasSetting -->

    <owl:ObjectProperty rdf:about="http://www.ontologydesignpatterns.org/ont/dul/DUL.owl#hasSetting">
        <owl:inverseOf rdf:resource="http://www.ontologydesignpatterns.org/ont/dul/DUL.owl#isSettingFor"/>
    </owl:ObjectProperty>
    


    <!-- http://www.ontologydesignpatterns.org/ont/dul/DUL.owl#includesEvent -->

    <owl:ObjectProperty rdf:about="http://www.ontologydesignpatterns.org/ont/dul/DUL.owl#includesEvent">
        <rdfs:subPropertyOf rdf:resource="http://www.ontologydesignpatterns.org/ont/dul/DUL.owl#isSettingFor"/>
        <owl:inverseOf rdf:resource="http://www.ontologydesignpatterns.org/ont/dul/DUL.owl#isEventIncludedIn"/>
        <rdfs:domain rdf:resource="http://www.ontologydesignpatterns.org/ont/dul/DUL.owl#Situation"/>
        <rdfs:comment>A relation between situations and events, e.g. &apos;this morning I&apos;ve prepared my coffee and had my fingers burnt&apos; (i.e.: the preparation of my coffee this morning included a burning of my fingers).</rdfs:comment>
        <rdfs:isDefinedBy rdf:resource="http://www.ontologydesignpatterns.org/ont/dul/DUL.owl"/>
        <rdfs:label xml:lang="en">includes event</rdfs:label>
    </owl:ObjectProperty>
    


    <!-- http://www.ontologydesignpatterns.org/ont/dul/DUL.owl#includesObject -->

    <owl:ObjectProperty rdf:about="http://www.ontologydesignpatterns.org/ont/dul/DUL.owl#includesObject">
        <rdfs:subPropertyOf rdf:resource="http://www.ontologydesignpatterns.org/ont/dul/DUL.owl#isSettingFor"/>
        <owl:inverseOf rdf:resource="http://www.ontologydesignpatterns.org/ont/dul/DUL.owl#isObjectIncludedIn"/>
        <rdfs:domain rdf:resource="http://www.ontologydesignpatterns.org/ont/dul/DUL.owl#Situation"/>
        <rdfs:range rdf:resource="http://www.ontologydesignpatterns.org/ont/dul/DUL.owl#Object"/>
        <rdfs:comment>A relation between situations and objects, e.g. &apos;this morning I&apos;ve prepared my coffee and had my fingers burnt&apos; (i.e.: the preparation of my coffee this morning included me).</rdfs:comment>
        <rdfs:isDefinedBy rdf:resource="http://www.ontologydesignpatterns.org/ont/dul/DUL.owl"/>
        <rdfs:label xml:lang="en">includes object</rdfs:label>
    </owl:ObjectProperty>
    


    <!-- http://www.ontologydesignpatterns.org/ont/dul/DUL.owl#includesTime -->

    <owl:ObjectProperty rdf:about="http://www.ontologydesignpatterns.org/ont/dul/DUL.owl#includesTime">
        <rdfs:subPropertyOf rdf:resource="http://www.ontologydesignpatterns.org/ont/dul/DUL.owl#isSettingFor"/>
        <owl:inverseOf rdf:resource="http://www.ontologydesignpatterns.org/ont/dul/DUL.owl#isTimeIncludedIn"/>
        <rdfs:domain rdf:resource="http://www.ontologydesignpatterns.org/ont/dul/DUL.owl#Situation"/>
        <rdfs:comment>A relation between situations and time intervals, e.g. &apos;this morning I&apos;ve prepared my coffee and had my fingers burnt&apos; (i.e.: preparing my coffee was held this morning). A data value attached to the time interval typically complements this modelling pattern.</rdfs:comment>
        <rdfs:isDefinedBy rdf:resource="http://www.ontologydesignpatterns.org/ont/dul/DUL.owl"/>
        <rdfs:label xml:lang="en">includes time</rdfs:label>
    </owl:ObjectProperty>
    


    <!-- http://www.ontologydesignpatterns.org/ont/dul/DUL.owl#isClassifiedBy -->

    <owl:ObjectProperty rdf:about="http://www.ontologydesignpatterns.org/ont/dul/DUL.owl#isClassifiedBy"/>
    


    <!-- http://www.ontologydesignpatterns.org/ont/dul/DUL.owl#isEventIncludedIn -->

    <owl:ObjectProperty rdf:about="http://www.ontologydesignpatterns.org/ont/dul/DUL.owl#isEventIncludedIn"/>
    


    <!-- http://www.ontologydesignpatterns.org/ont/dul/DUL.owl#isObjectIncludedIn -->

    <owl:ObjectProperty rdf:about="http://www.ontologydesignpatterns.org/ont/dul/DUL.owl#isObjectIncludedIn"/>
    


    <!-- http://www.ontologydesignpatterns.org/ont/dul/DUL.owl#isPartOf -->

    <owl:ObjectProperty rdf:about="http://www.ontologydesignpatterns.org/ont/dul/DUL.owl#isPartOf">
        <rdfs:subPropertyOf rdf:resource="http://www.ontologydesignpatterns.org/ont/dul/DUL.owl#associatedWith"/>
        <rdf:type rdf:resource="http://www.w3.org/2002/07/owl#TransitiveProperty"/>
        <rdf:type rdf:resource="http://www.w3.org/2002/07/owl#ReflexiveProperty"/>
        <rdfs:domain rdf:resource="http://www.ontologydesignpatterns.org/ont/dul/DUL.owl#Entity"/>
        <rdfs:range rdf:resource="http://www.ontologydesignpatterns.org/ont/dul/DUL.owl#Entity"/>
        <rdfs:comment>A relation between any entities, e.g. &apos;brain is a part of the human body&apos;. See dul:hasPart for additional documentation.</rdfs:comment>
        <rdfs:isDefinedBy rdf:resource="http://www.ontologydesignpatterns.org/ont/dul/DUL.owl"/>
        <rdfs:label xml:lang="en">is part of</rdfs:label>
    </owl:ObjectProperty>
    


    <!-- http://www.ontologydesignpatterns.org/ont/dul/DUL.owl#isSatisfiedBy -->

    <owl:ObjectProperty rdf:about="http://www.ontologydesignpatterns.org/ont/dul/DUL.owl#isSatisfiedBy">
        <owl:inverseOf rdf:resource="http://www.ontologydesignpatterns.org/ont/dul/DUL.owl#satisfies"/>
    </owl:ObjectProperty>
    


    <!-- http://www.ontologydesignpatterns.org/ont/dul/DUL.owl#isSettingFor -->

    <owl:ObjectProperty rdf:about="http://www.ontologydesignpatterns.org/ont/dul/DUL.owl#isSettingFor">
        <rdfs:subPropertyOf rdf:resource="http://www.ontologydesignpatterns.org/ont/dul/DUL.owl#associatedWith"/>
        <rdfs:domain rdf:resource="http://www.ontologydesignpatterns.org/ont/dul/DUL.owl#Situation"/>
        <rdfs:range rdf:resource="http://www.ontologydesignpatterns.org/ont/dul/DUL.owl#Entity"/>
        <rdfs:comment>A relation between situations and entities, e.g. &apos;this morning I&apos;ve prepared my coffee with a new fantastic Arabica&apos;, i.e.: the preparation of my coffee this morning is the setting for (an amount of) a new fantastic Arabica.</rdfs:comment>
        <rdfs:isDefinedBy rdf:resource="http://www.ontologydesignpatterns.org/ont/dul/DUL.owl"/>
        <rdfs:label xml:lang="en">is setting for</rdfs:label>
    </owl:ObjectProperty>
    


    <!-- http://www.ontologydesignpatterns.org/ont/dul/DUL.owl#isTimeIncludedIn -->

    <owl:ObjectProperty rdf:about="http://www.ontologydesignpatterns.org/ont/dul/DUL.owl#isTimeIncludedIn"/>
    


    <!-- http://www.ontologydesignpatterns.org/ont/dul/DUL.owl#precedes -->

    <owl:ObjectProperty rdf:about="http://www.ontologydesignpatterns.org/ont/dul/DUL.owl#precedes">
        <rdfs:subPropertyOf rdf:resource="http://www.ontologydesignpatterns.org/ont/dul/DUL.owl#associatedWith"/>
        <rdf:type rdf:resource="http://www.w3.org/2002/07/owl#TransitiveProperty"/>
        <rdfs:domain rdf:resource="http://www.ontologydesignpatterns.org/ont/dul/DUL.owl#Entity"/>
        <rdfs:range rdf:resource="http://www.ontologydesignpatterns.org/ont/dul/DUL.owl#Entity"/>
        <rdfs:comment>A relation between entities, expressing a &apos;sequence&apos; schema. 
E.g. &apos;year 1999 precedes 2000&apos;, &apos;deciding what coffee to use&apos; precedes &apos;preparing coffee&apos;, &apos;World War II follows World War I&apos;, &apos;in the Milan to Rome autoroute, Bologna precedes Florence&apos;, etc.
It can then be used between tasks, processes, time intervals, spatially locate objects, situations, etc. 
Subproperties can be defined in order to distinguish the different uses.</rdfs:comment>
        <rdfs:isDefinedBy rdf:resource="http://www.ontologydesignpatterns.org/ont/dul/DUL.owl"/>
        <rdfs:label xml:lang="en">precedes</rdfs:label>
    </owl:ObjectProperty>
    


    <!-- http://www.ontologydesignpatterns.org/ont/dul/DUL.owl#satisfies -->

    <owl:ObjectProperty rdf:about="http://www.ontologydesignpatterns.org/ont/dul/DUL.owl#satisfies">
        <rdfs:subPropertyOf rdf:resource="http://www.ontologydesignpatterns.org/ont/dul/DUL.owl#associatedWith"/>
        <rdfs:domain rdf:resource="http://www.ontologydesignpatterns.org/ont/dul/DUL.owl#Situation"/>
        <rdfs:range rdf:resource="http://www.ontologydesignpatterns.org/ont/dul/DUL.owl#Description"/>
        <rdfs:comment>A relation between a Situation and a Description, e.g. the execution of a Plan satisfies that plan.</rdfs:comment>
        <rdfs:isDefinedBy rdf:resource="http://www.ontologydesignpatterns.org/ont/dul/DUL.owl"/>
        <rdfs:label xml:lang="en">satisfies</rdfs:label>
    </owl:ObjectProperty>
    


    <!-- http://www.w3.org/2006/time#after -->

    <owl:ObjectProperty rdf:about="http://www.w3.org/2006/time#after">
        <owl:inverseOf rdf:resource="http://www.w3.org/2006/time#before"/>
        <rdfs:domain rdf:resource="http://www.w3.org/2006/time#TemporalEntity"/>
        <rdfs:range rdf:resource="http://www.w3.org/2006/time#TemporalEntity"/>
        <rdfs:comment xml:lang="en">Gives directionality to time. If a temporal entity T1 is after another temporal entity T2, then the beginning of T1 is after the end of T2. </rdfs:comment>
        <rdfs:label xml:lang="en">after</rdfs:label>
    </owl:ObjectProperty>
    


    <!-- http://www.w3.org/2006/time#before -->

    <owl:ObjectProperty rdf:about="http://www.w3.org/2006/time#before">
        <rdfs:domain rdf:resource="http://www.w3.org/2006/time#TemporalEntity"/>
        <rdfs:range rdf:resource="http://www.w3.org/2006/time#TemporalEntity"/>
        <rdfs:comment xml:lang="en">Gives directionality to time. If a temporal entity T1 is before another temporal entity T2, then the end of T1 is before the beginning of T2. Thus, &quot;before&quot; can be considered to be basic to instants and derived for intervals</rdfs:comment>
        <rdfs:label xml:lang="en">before</rdfs:label>
    </owl:ObjectProperty>
    


    <!-- http://www.w3.org/2006/time#hasBeginnging -->

    <owl:ObjectProperty rdf:about="http://www.w3.org/2006/time#hasBeginnging">
        <rdfs:subPropertyOf rdf:resource="http://www.w3.org/2006/time#hasTime"/>
        <rdfs:domain rdf:resource="http://www.w3.org/2006/time#TemporalEntity"/>
        <rdfs:range rdf:resource="http://www.w3.org/2006/time#Instant"/>
        <rdfs:comment xml:lang="en">Beginning of a temporal entity</rdfs:comment>
        <rdfs:label xml:lang="en">has beginning</rdfs:label>
    </owl:ObjectProperty>
    


    <!-- http://www.w3.org/2006/time#hasEnd -->

    <owl:ObjectProperty rdf:about="http://www.w3.org/2006/time#hasEnd">
        <rdfs:subPropertyOf rdf:resource="http://www.w3.org/2006/time#hasTime"/>
        <rdfs:domain rdf:resource="http://www.w3.org/2006/time#TemporalEntity"/>
        <rdfs:range rdf:resource="http://www.w3.org/2006/time#Instant"/>
        <rdfs:comment xml:lang="en">End of a temporal entity</rdfs:comment>
        <rdfs:label xml:lang="en">has end</rdfs:label>
    </owl:ObjectProperty>
    


    <!-- http://www.w3.org/2006/time#hasTime -->

    <owl:ObjectProperty rdf:about="http://www.w3.org/2006/time#hasTime"/>
    


    <!-- https://ontology.swissartresearch.net/aaao/ZP111_initiated -->

    <owl:ObjectProperty rdf:about="https://ontology.swissartresearch.net/aaao/ZP111_initiated">
        <rdfs:domain rdf:resource="http://www.cidoc-crm.org/cidoc-crm/E5_Event"/>
        <rdfs:range rdf:resource="https://ontology.swissartresearch.net/aaao/ZE1_Institutional_Fact"/>
        <rdfs:comment xml:lang="en">This property is used to connect the instance of event to the instance of institutional fact which it brought into existence by fiat thanks to its accordance to a socially defined norm. In this case the bringing about of a new institutional fact need not be intentional or following any particular rule intentionally. Rather, within a social context it is recognized that the very fact of a particular event occurring is causal to the initiation of the related social fact. For example, in certain property right laws, the very fact of writing down an idea (E65 Creation) initiates an instance of property right over the generated information object, regardless of the intention or not of the author to so create such a right.</rdfs:comment>
        <rdfs:label xml:lang="en">initiated</rdfs:label>
        <skos:notation>ZP111</skos:notation>
    </owl:ObjectProperty>
    


    <!-- https://ontology.swissartresearch.net/aaao/ZP112_terminated -->

    <owl:ObjectProperty rdf:about="https://ontology.swissartresearch.net/aaao/ZP112_terminated">
        <rdfs:domain rdf:resource="http://www.cidoc-crm.org/cidoc-crm/E5_Event"/>
        <rdfs:range rdf:resource="https://ontology.swissartresearch.net/aaao/ZE1_Institutional_Fact"/>
        <rdfs:comment xml:lang="en">This property is used to connect the instance of event to the instance of institutional fact which it terminated the existence of by fiat thanks to its accordance to a socially defined norm. In this case the cancellation of an institutional fact need not be intentional or following any particular rule intentionally. Rather, within a social context it is recognized that the very fact of a particular event occurring is causal to the cancellation of the related social fact. For example, a certain social system may recognize that an &apos;&apos;act of god&apos;&apos; such as an earthquake may terminate the property right of an individual over some object (another social system may not, however).</rdfs:comment>
        <rdfs:label xml:lang="en">terminated</rdfs:label>
        <skos:notation>ZP112</skos:notation>
    </owl:ObjectProperty>
    


    <!-- https://ontology.swissartresearch.net/aaao/ZP113_has_successor_status -->

    <owl:ObjectProperty rdf:about="https://ontology.swissartresearch.net/aaao/ZP113_has_successor_status">
        <rdfs:domain rdf:resource="https://ontology.swissartresearch.net/aaao/ZE1_Institutional_Fact"/>
        <rdfs:range rdf:resource="https://ontology.swissartresearch.net/aaao/ZE1_Institutional_Fact"/>
        <rdfs:comment xml:lang="en">This property links one instance of institutional fact with another where the latter succeeds the former as a formal continuation.</rdfs:comment>
        <rdfs:label xml:lang="en">has successor status</rdfs:label>
        <skos:notation>ZP113</skos:notation>
    </owl:ObjectProperty>
    


    <!-- https://ontology.swissartresearch.net/aaao/ZP115_holds_over -->

    <owl:ObjectProperty rdf:about="https://ontology.swissartresearch.net/aaao/ZP115_holds_over">
        <rdfs:domain rdf:resource="https://ontology.swissartresearch.net/aaao/ZE1_Institutional_Fact"/>
        <rdfs:range rdf:resource="https://ontology.swissartresearch.net/aaao/ZE37_Population"/>
        <rdfs:comment xml:lang="en">This property associates and instance of institutional fact to an instance of population over which this fact holds. As opposed to the property of ZP4 holding for, the effect which this institutional fact holds in relation to the related population is not necessarily one which has been directly intended. The population undergoes the social fact instantiated, rather than causing it to occur directly through agency in a speech act or transformative act. The population is the patient of this operation, not its agent.</rdfs:comment>
        <rdfs:label xml:lang="en">holds over</rdfs:label>
        <skos:notation>ZP115</skos:notation>
    </owl:ObjectProperty>
    


    <!-- https://ontology.swissartresearch.net/aaao/ZP11_has_classificatory_subject -->

    <owl:ObjectProperty rdf:about="https://ontology.swissartresearch.net/aaao/ZP11_has_classificatory_subject">
        <rdfs:subPropertyOf rdf:resource="https://ontology.swissartresearch.net/aaao/ZP1_has_intentional_subject"/>
        <rdfs:domain rdf:resource="https://ontology.swissartresearch.net/aaao/ZE4_Classificatory_Status"/>
        <rdfs:range rdf:resource="http://www.cidoc-crm.org/cidoc-crm/E1_CRM_Entity"/>
        <rdfs:comment xml:lang="en">This property is used to indicate the entity for which a certain classification is taken to hold by the instance of classificatory status.

 
</rdfs:comment>
        <rdfs:label xml:lang="en">has classificatory subject</rdfs:label>
        <skos:notation>ZP11</skos:notation>
    </owl:ObjectProperty>
    


    <!-- https://ontology.swissartresearch.net/aaao/ZP12_ascribes_classification -->

    <owl:ObjectProperty rdf:about="https://ontology.swissartresearch.net/aaao/ZP12_ascribes_classification">
        <rdfs:subPropertyOf rdf:resource="https://ontology.swissartresearch.net/aaao/ZP2_ascribes_intentional_target"/>
        <rdfs:domain rdf:resource="https://ontology.swissartresearch.net/aaao/ZE4_Classificatory_Status"/>
        <rdfs:range rdf:resource="http://www.cidoc-crm.org/cidoc-crm/E55_Type"/>
        <rdfs:comment xml:lang="en">This property is used to indicate the type which is indicated as holding for the subject of the classification status.

 
</rdfs:comment>
        <rdfs:label xml:lang="en">ascribes classification</rdfs:label>
        <skos:notation>ZP12</skos:notation>
    </owl:ObjectProperty>
    


    <!-- https://ontology.swissartresearch.net/aaao/ZP13_ascribes_classification_relation -->

    <owl:ObjectProperty rdf:about="https://ontology.swissartresearch.net/aaao/ZP13_ascribes_classification_relation"/>
    


    <!-- https://ontology.swissartresearch.net/aaao/ZP14_has_functional_subject -->

    <owl:ObjectProperty rdf:about="https://ontology.swissartresearch.net/aaao/ZP14_has_functional_subject">
        <rdfs:subPropertyOf rdf:resource="https://ontology.swissartresearch.net/aaao/ZP11_has_classificatory_subject"/>
        <rdfs:domain rdf:resource="https://ontology.swissartresearch.net/aaao/ZE5_Function_Status"/>
        <rdfs:range rdf:resource="http://www.cidoc-crm.org/cidoc-crm/E1_CRM_Entity"/>
        <rdfs:comment xml:lang="en">This property is used to indicate the entity for which a certain functional classification is taken to hold by the instance of functional status.</rdfs:comment>
        <rdfs:comment xml:lang="en">This property is used to indicate the entity for which a certain functional classification is taken to hold by the instance of functional status.

 
</rdfs:comment>
        <rdfs:label xml:lang="en">has functional subject</rdfs:label>
        <skos:notation>ZP14</skos:notation>
    </owl:ObjectProperty>
    


    <!-- https://ontology.swissartresearch.net/aaao/ZP15_ascribes_function -->

    <owl:ObjectProperty rdf:about="https://ontology.swissartresearch.net/aaao/ZP15_ascribes_function">
        <rdfs:subPropertyOf rdf:resource="https://ontology.swissartresearch.net/aaao/ZP12_ascribes_classification"/>
        <rdfs:domain rdf:resource="https://ontology.swissartresearch.net/aaao/ZE5_Function_Status"/>
        <rdfs:range rdf:resource="http://www.cidoc-crm.org/cidoc-crm/E55_Type"/>
        <rdfs:comment xml:lang="en">This property is used to indicate the type of function which is indicated as holding for the subject of the function status.

 
</rdfs:comment>
        <rdfs:label xml:lang="en">ascribes function</rdfs:label>
        <skos:notation>ZP15</skos:notation>
    </owl:ObjectProperty>
    


    <!-- https://ontology.swissartresearch.net/aaao/ZP16_ascribes_functional_relation -->

    <owl:ObjectProperty rdf:about="https://ontology.swissartresearch.net/aaao/ZP16_ascribes_functional_relation">
        <rdfs:subPropertyOf rdf:resource="https://ontology.swissartresearch.net/aaao/ZP13_ascribes_classification_relation"/>
        <rdfs:domain rdf:resource="https://ontology.swissartresearch.net/aaao/ZE5_Function_Status"/>
        <rdfs:range rdf:resource="http://www.cidoc-crm.org/cidoc-crm/E55_Type"/>
        <rdfs:comment xml:lang="en">This property is used to indicate the specific manner in which the function which is indicated as holding for the subject of the function status pertains to this subject.

 
</rdfs:comment>
        <rdfs:label xml:lang="en">ascribes functional relation</rdfs:label>
        <skos:notation>ZP16</skos:notation>
    </owl:ObjectProperty>
    


    <!-- https://ontology.swissartresearch.net/aaao/ZP1_has_intentional_subject -->

    <owl:ObjectProperty rdf:about="https://ontology.swissartresearch.net/aaao/ZP1_has_intentional_subject"/>
    


    <!-- https://ontology.swissartresearch.net/aaao/ZP2_ascribes_intentional_target -->

    <owl:ObjectProperty rdf:about="https://ontology.swissartresearch.net/aaao/ZP2_ascribes_intentional_target"/>
    


    <!-- https://ontology.swissartresearch.net/aaao/ZP4_holds_for -->

    <owl:ObjectProperty rdf:about="https://ontology.swissartresearch.net/aaao/ZP4_holds_for">
        <rdfs:domain rdf:resource="https://ontology.swissartresearch.net/aaao/ZE1_Institutional_Fact"/>
        <rdfs:range rdf:resource="http://www.cidoc-crm.org/cidoc-crm/E74_Group"/>
        <rdfs:comment xml:lang="en">This property is used to indicate the community or group for whom an instance of institutional fact holds. Institutional facts have identity only relative to some group for whom they have a significance as formulated through a chosen symbolic system.</rdfs:comment>
        <rdfs:comment xml:lang="en">This property is used to indicate the community or group for whom an instance of institutional fact holds. Institutional facts have identity only relative to some group for whom they have a significance as formulated through a chosen symbolic system. </rdfs:comment>
        <rdfs:label xml:lang="en">ZP4 holds for</rdfs:label>
        <rdfs:label xml:lang="en">holds for</rdfs:label>
        <skos:notation>ZP4</skos:notation>
    </owl:ObjectProperty>
    


    <!-- https://ontology.swissartresearch.net/aaao/ZP75_applies_for_context -->

    <owl:ObjectProperty rdf:about="https://ontology.swissartresearch.net/aaao/ZP75_applies_for_context">
        <rdfs:domain rdf:resource="https://ontology.swissartresearch.net/aaao/ZE1_Institutional_Fact"/>
        <rdfs:range rdf:resource="http://www.cidoc-crm.org/cidoc-crm/E5_Event"/>
        <rdfs:comment xml:lang="en">This property is used to indicate an event context which limits the temporal scope within which an instance of institutional fact is meant to hold. When indicated the event context stands as the frame in which the institutional fact is held to be valid by the associated group for whom it has significance.</rdfs:comment>
        <rdfs:label xml:lang="en">ZP75 applies for context (is context for)</rdfs:label>
        <rdfs:label xml:lang="en">applies for context</rdfs:label>
        <skos:notation>ZP75</skos:notation>
    </owl:ObjectProperty>
    


    <!-- https://ontology.swissartresearch.net/aaao/ZP76_applies_for_context_type -->

    <owl:ObjectProperty rdf:about="https://ontology.swissartresearch.net/aaao/ZP76_applies_for_context_type">
        <rdfs:domain rdf:resource="https://ontology.swissartresearch.net/aaao/ZE1_Institutional_Fact"/>
        <rdfs:range rdf:resource="http://www.cidoc-crm.org/cidoc-crm/E55_Type"/>
        <rdfs:comment xml:lang="en">This property is used to indicate an event context type which limits the spatio-temporal scope within which an instance of institutional fact is meant to hold to certain kinds of event. When indicated the event context type stands as the frame or frames in which the institutional fact is held to be valid by the associated group for whom it has significance.</rdfs:comment>
        <rdfs:label xml:lang="en">applies for context type</rdfs:label>
        <skos:notation>ZP76</skos:notation>
    </owl:ObjectProperty>
    


    <!-- https://periodo.github.io/edtf-ontology/edtfo.ttl#hasEDTFDateTimeDescription -->

    <owl:ObjectProperty rdf:about="https://periodo.github.io/edtf-ontology/edtfo.ttl#hasEDTFDateTimeDescription">
        <rdfs:domain rdf:resource="http://www.w3.org/2006/time#Interval"/>
        <rdfs:range rdf:resource="http://id.loc.gov/datatypes/edtf/EDTF"/>
    </owl:ObjectProperty>
    


    <!-- https://periodo.github.io/edtf-ontology/edtfo.ttl#inEDTFDateTime -->

    <owl:ObjectProperty rdf:about="https://periodo.github.io/edtf-ontology/edtfo.ttl#inEDTFDateTime">
        <rdfs:domain rdf:resource="http://www.w3.org/2006/time#Instant"/>
        <rdfs:range rdf:resource="http://id.loc.gov/datatypes/edtf/EDTF"/>
    </owl:ObjectProperty>
    


    <!-- https://w3id.org/chint/evo/createsPhysicalVersion -->

    <owl:ObjectProperty rdf:about="https://w3id.org/chint/evo/createsPhysicalVersion">
        <rdfs:domain rdf:resource="http://www.cidoc-crm.org/cidoc-crm/E11_Modification"/>
        <rdfs:range rdf:resource="http://www.cidoc-crm.org/cidoc-crm/E24_Physical_Human-Made_Thing"/>
        <rdfs:comment xml:lang="en">The property relates the crm:E11 Modification to the physical version resulting from the intervention</rdfs:comment>
    </owl:ObjectProperty>
    


    <!-- https://w3id.org/chint/ois/hasTimePeriod -->

    <owl:ObjectProperty rdf:about="https://w3id.org/chint/ois/hasTimePeriod">
        <rdfs:domain rdf:resource="https://w3id.org/chint/ois/ObjectInRecurrentEvent"/>
        <rdfs:comment xml:lang="en">Property relating a recurrent event series to the time frequency with which it occurs. It belongs to the Time Period Pattern, not imported because currently not available</rdfs:comment>
    </owl:ObjectProperty>
    


    <!-- https://w3id.org/chint/ontology/believedThing -->

    <owl:ObjectProperty rdf:about="https://w3id.org/chint/ontology/believedThing">
        <rdfs:domain rdf:resource="https://w3id.org/icon/ontology/Belief"/>
        <rdfs:range rdf:resource="http://www.w3.org/2002/07/owl#Thing"/>
        <rdfs:comment>A relation specifying the thing believed in the belief system of the culture in question.</rdfs:comment>
        <rdfs:label>believed thing</rdfs:label>
    </owl:ObjectProperty>
    


    <!-- https://w3id.org/chint/ontology/conceptuallyModifies -->

    <owl:ObjectProperty rdf:about="https://w3id.org/chint/ontology/conceptuallyModifies">
        <rdfs:domain rdf:resource="https://w3id.org/chint/ontology/ConceptualVariation"/>
        <rdfs:range rdf:resource="http://www.cidoc-crm.org/cidoc-crm/E36_Visual_Item"/>
        <rdfs:comment xml:lang="en">The property relates the :ConceptualVariation to the Visual Item it modifies, i.e., the version of the work before the intervention</rdfs:comment>
    </owl:ObjectProperty>
    


    <!-- https://w3id.org/chint/ontology/createsConceptualVersion -->

    <owl:ObjectProperty rdf:about="https://w3id.org/chint/ontology/createsConceptualVersion">
        <rdfs:domain rdf:resource="https://w3id.org/chint/ontology/ConceptualVariation"/>
        <rdfs:range rdf:resource="http://www.cidoc-crm.org/cidoc-crm/E36_Visual_Item"/>
        <rdfs:comment xml:lang="en">The property relates the :ConceptualVariation to the Visual Item version resulting from intervention</rdfs:comment>
    </owl:ObjectProperty>
    


    <!-- https://w3id.org/chint/ontology/hasContext -->

    <owl:ObjectProperty rdf:about="https://w3id.org/chint/ontology/hasContext">
        <rdfs:domain rdf:resource="http://www.w3.org/2002/07/owl#Thing"/>
        <rdfs:range rdf:resource="https://w3id.org/chint/ontology/HistoricalFrame"/>
        <rdfs:comment xml:lang="en">Generic relation that expresses that an entity motivates the existence or characteristics of another one (e.g., the belief that St. Servatius drunk from the cup motivates the healing function of the cup)</rdfs:comment>
        <rdfs:label>has context</rdfs:label>
    </owl:ObjectProperty>
    


    <!-- https://w3id.org/chint/ontology/hasCreationContext -->

    <owl:ObjectProperty rdf:about="https://w3id.org/chint/ontology/hasCreationContext">
        <rdfs:subPropertyOf rdf:resource="https://w3id.org/chint/ontology/hasContext"/>
        <rdfs:domain rdf:resource="http://www.w3.org/2002/07/owl#Thing"/>
        <rdfs:range rdf:resource="https://w3id.org/chint/ontology/HistoricalFrame"/>
        <rdfs:comment>Subproperty of :hasContext to specifically express that the object examined is related to the cultural context in which it was created (e.g., “Roman culture, is the creation context of the Roman cup created in I Century)</rdfs:comment>
        <rdfs:label xml:lang="en">has creation context</rdfs:label>
    </owl:ObjectProperty>
    


    <!-- https://w3id.org/chint/ontology/hasFunction -->

    <owl:ObjectProperty rdf:about="https://w3id.org/chint/ontology/hasFunction">
        <rdfs:subPropertyOf rdf:resource="http://www.cidoc-crm.org/cidoc-crm/P2_has_type"/>
        <rdfs:domain rdf:resource="http://www.cidoc-crm.org/cidoc-crm/E70_Thing"/>
        <rdfs:range rdf:resource="http://www.cidoc-crm.org/cidoc-crm/E55_Type"/>
        <rdfs:comment xml:lang="en">Property expressing the function that a CH object has. It is a shortcut for the longer path aaao:ZE5_Function Status aaao:ZP14_has_functional_subject crm:E1_Entity; aaao:ZP15 _ascribes_function crm:E55_Type. It is declared as subroperty of crm:P2_has_type and as a superproprerty of crm:P103_was_intended_forand crm:P101_had_as_general_use, which add more detail to the usage or function that the object has.</rdfs:comment>
        <rdfs:label xml:lang="en">has function</rdfs:label>
    </owl:ObjectProperty>
    


    <!-- https://w3id.org/chint/ontology/hasMemberEvent -->

    <owl:ObjectProperty rdf:about="https://w3id.org/chint/ontology/hasMemberEvent">
        <rdfs:domain rdf:resource="https://w3id.org/chint/ontology/ObjectInRecurrentEvent"/>
        <rdfs:comment xml:lang="en">Property to indicate the events of a series</rdfs:comment>
        <rdfs:label xml:lang="en">has member event</rdfs:label>
    </owl:ObjectProperty>
    


    <!-- https://w3id.org/chint/ontology/hasUnifyingFactor -->

    <owl:ObjectProperty rdf:about="https://w3id.org/chint/ontology/hasUnifyingFactor">
        <rdfs:domain rdf:resource="https://w3id.org/chint/ontology/ObjectInRecurrentEvent"/>
        <rdfs:range rdf:resource="http://www.w3.org/2002/07/owl#Thing"/>
        <rdfs:comment xml:lang="en">Property indicating the unifying factors of a collection of events repeating over time (e.g., the same place)</rdfs:comment>
        <rdfs:comment xml:lang="en">has unifying factor</rdfs:comment>
    </owl:ObjectProperty>
    


    <!-- https://w3id.org/chint/ontology/includesCulturalTrait -->

    <owl:ObjectProperty rdf:about="https://w3id.org/chint/ontology/includesCulturalTrait">
        <rdfs:domain rdf:resource="https://w3id.org/chint/ontology/HistoricalFrame"/>
        <rdfs:range rdf:resource="https://w3id.org/icon/ontology/CulturalPhenomenon"/>
        <rdfs:comment xml:lang="en">The property relates a Historical Frame with the immaterial traits of a culture that are relevant for the understanding of the objects. Once ontologies for societal aspects (e.g., SDHSS) will be fully worked out, the range of this property will be updated.</rdfs:comment>
        <rdfs:label xml:lang="en">includes cultural trait</rdfs:label>
    </owl:ObjectProperty>
    


    <!-- https://w3id.org/chint/ontology/includesEventsOfType -->

    <owl:ObjectProperty rdf:about="https://w3id.org/chint/ontology/includesEventsOfType">
        <rdfs:domain rdf:resource="https://w3id.org/chint/ontology/ObjectInRecurrentEvent"/>
        <rdfs:range rdf:resource="http://www.ontologydesignpatterns.org/ont/dul/DUL.owl#EventType"/>
        <rdfs:comment xml:lang="en">Relate the event series with the type of event that is included (e.g., mass, procession).</rdfs:comment>
        <rdfs:label xml:lang="en">includes events of type</rdfs:label>
    </owl:ObjectProperty>
    


    <!-- https://w3id.org/chint/ontology/includesFact -->

    <owl:ObjectProperty rdf:about="https://w3id.org/chint/ontology/includesFact">
        <rdfs:subPropertyOf rdf:resource="http://www.ontologydesignpatterns.org/ont/dul/DUL.owl#isSettingFor"/>
        <rdfs:domain rdf:resource="https://w3id.org/chint/ontology/ObjectInRecurrentEvent"/>
        <rdfs:range rdf:resource="https://ontology.swissartresearch.net/aaao/ZE1_Institutional_Fact"/>
        <rdfs:comment xml:lang="en">Property expressing the fact that the indicated institutional fact (for example, the fact that the CH object holds a function) is included in the situation that represents a series of events repeating over time.</rdfs:comment>
    </owl:ObjectProperty>
    


    <!-- https://w3id.org/chint/ontology/manifestsIn -->

    <owl:ObjectProperty rdf:about="https://w3id.org/chint/ontology/manifestsIn">
        <rdfs:domain rdf:resource="http://www.cidoc-crm.org/cidoc-crm/E24_Physical_Human-Made_Thing"/>
        <rdfs:range rdf:resource="http://www.cidoc-crm.org/cidoc-crm/E24_Physical_Human-Made_Thing"/>
        <rdfs:comment xml:lang="en">The property relates a CH artifact to the physical versions that are created by a physical act that consistently modifies the artifact but without affecting its identity. It is the result of the action of a crm:E81_Transformation that generates a new version of the item (and not a fully new item).</rdfs:comment>
    </owl:ObjectProperty>
    


    <!-- https://w3id.org/chint/ontology/motivates -->

    <owl:ObjectProperty rdf:about="https://w3id.org/chint/ontology/motivates">
        <rdfs:domain rdf:resource="http://www.cidoc-crm.org/cidoc-crm/E1_CRM_Entity"/>
        <rdfs:range rdf:resource="http://www.cidoc-crm.org/cidoc-crm/E1_CRM_Entity"/>
        <rdfs:comment xml:lang="en">Generic relation that expresses that an entity motivates the existence or characteristics of another one (e.g., the belief that St. Servatius drunk from the cup motivates the healing function of the cup)</rdfs:comment>
        <rdfs:label>motivates</rdfs:label>
    </owl:ObjectProperty>
    


    <!-- https://w3id.org/chint/ontology/refersToCulture -->

    <owl:ObjectProperty rdf:about="https://w3id.org/chint/ontology/refersToCulture">
        <rdfs:domain rdf:resource="https://w3id.org/chint/ontology/HistoricalFrame"/>
        <rdfs:range rdf:resource="https://w3id.org/chint/ontology/Culture"/>
        <rdfs:comment xml:lang="en">Relation of historical frame to the fuzzy culture it observes</rdfs:comment>
        <rdfs:label>refers to culture</rdfs:label>
    </owl:ObjectProperty>
    


    <!-- 
    ///////////////////////////////////////////////////////////////////////////////////////
    //
    // Data properties
    //
    ///////////////////////////////////////////////////////////////////////////////////////
     -->

    


    <!-- https://periodo.github.io/edtf-ontology/edtfo.ttl#hasEDTFDateTimeDescription -->

    <owl:DatatypeProperty rdf:about="https://periodo.github.io/edtf-ontology/edtfo.ttl#hasEDTFDateTimeDescription"/>
    


    <!-- https://periodo.github.io/edtf-ontology/edtfo.ttl#inEDTFDateTime -->

    <owl:DatatypeProperty rdf:about="https://periodo.github.io/edtf-ontology/edtfo.ttl#inEDTFDateTime"/>
    


    <!-- 
    ///////////////////////////////////////////////////////////////////////////////////////
    //
    // Classes
    //
    ///////////////////////////////////////////////////////////////////////////////////////
     -->

    


    <!-- http://data.odeuropa.eu/ontology/L11_Smell -->

    <owl:Class rdf:about="http://data.odeuropa.eu/ontology/L11_Smell">
        <rdfs:subClassOf rdf:resource="http://data.odeuropa.eu/ontology/L1_Sensory_Stimulus"/>
        <rdfs:comment xml:lang="en">This class comprises all olfactory stimuli, or smells, considered as unique and un-repeatable, possibly existing in a specific time and place, to not be confused with possible generalisation.

Example:
* The smell of a specific rose in my garden in a rainy day (and not the general smell of roses)</rdfs:comment>
    </owl:Class>
    


    <!-- http://data.odeuropa.eu/ontology/L12_Smell_Emission -->

    <owl:Class rdf:about="http://data.odeuropa.eu/ontology/L12_Smell_Emission">
        <rdfs:subClassOf rdf:resource="http://data.odeuropa.eu/ontology/L2_Stimulus_Generation"/>
        <rdfs:comment xml:lang="en">This class comprises events in which a specific smell has been generated, either by human intervention or because of natural phenomena.

Examples:
* The eruption of Vesuvius in 79 d.C. emitted sulphuric smells (Pliny the Younger, Epistulae)
* A perfumed candle is emitting good smell of lavender</rdfs:comment>
    </owl:Class>
    


    <!-- http://data.odeuropa.eu/ontology/L13_Olfactory_Experience -->

    <owl:Class rdf:about="http://data.odeuropa.eu/ontology/L13_Olfactory_Experience">
        <rdfs:subClassOf rdf:resource="http://data.odeuropa.eu/ontology/L3_Sensory_Experience"/>
        <rdfs:comment xml:lang="en">This class comprises activities in which an actor (human or animal) is perceiving a smell</rdfs:comment>
    </owl:Class>
    


    <!-- http://data.odeuropa.eu/ontology/L1_Sensory_Stimulus -->

    <owl:Class rdf:about="http://data.odeuropa.eu/ontology/L1_Sensory_Stimulus"/>
    


    <!-- http://data.odeuropa.eu/ontology/L2_Stimulus_Generation -->

    <owl:Class rdf:about="http://data.odeuropa.eu/ontology/L2_Stimulus_Generation"/>
    


    <!-- http://data.odeuropa.eu/ontology/L3_Sensory_Experience -->

    <owl:Class rdf:about="http://data.odeuropa.eu/ontology/L3_Sensory_Experience"/>
    


    <!-- http://id.loc.gov/datatypes/edtf/EDTF -->

    <owl:Class rdf:about="http://id.loc.gov/datatypes/edtf/EDTF">
        <rdfs:label xml:lang="en">Extended Date/Time Format</rdfs:label>
        <skos:definition xml:lang="en">This datatype describes dates, dates and times,
and intervals that adhere to features of any of EDTF Levels 0, 1, or
2.</skos:definition>
    </owl:Class>
    


    <!-- http://www.cidoc-crm.org/cidoc-crm/E11_Modification -->

    <owl:Class rdf:about="http://www.cidoc-crm.org/cidoc-crm/E11_Modification"/>
    


    <!-- http://www.cidoc-crm.org/cidoc-crm/E18_Physical_Thing -->

    <owl:Class rdf:about="http://www.cidoc-crm.org/cidoc-crm/E18_Physical_Thing"/>
    


    <!-- http://www.cidoc-crm.org/cidoc-crm/E1_CRM_Entity -->

    <owl:Class rdf:about="http://www.cidoc-crm.org/cidoc-crm/E1_CRM_Entity"/>
    


    <!-- http://www.cidoc-crm.org/cidoc-crm/E20_Biological_Object -->

    <owl:Class rdf:about="http://www.cidoc-crm.org/cidoc-crm/E20_Biological_Object"/>
    


    <!-- http://www.cidoc-crm.org/cidoc-crm/E21_Person -->

    <owl:Class rdf:about="http://www.cidoc-crm.org/cidoc-crm/E21_Person">
        <rdfs:subClassOf rdf:resource="http://www.cidoc-crm.org/cidoc-crm/E20_Biological_Object"/>
        <rdfs:subClassOf rdf:resource="http://www.cidoc-crm.org/cidoc-crm/E39_Actor"/>
        <rdfs:comment>This class comprises real persons who live or are assumed to have lived. Legendary figures that may have existed, such as Ulysses and King Arthur, fall into this class if the documentation refers to them as historical figures. In cases where doubt exists as to whether several persons are in fact identical, multiple instances can be created and linked to indicate their relationship. The CIDOC CRM does not propose a specific form to support reasoning about possible identity.In a bibliographic context, a name presented following the conventions usually employed for personal names will be assumed to correspond to an actual real person (an instance of E21 Person), unless evidence is available to indicate that this is not the case. The fact that a persona may erroneously be classified as an instance of E21 Person does not imply that the concept comprises personae. </rdfs:comment>
        <rdfs:label xml:lang="en">Person</rdfs:label>
        <skos:notation>E21</skos:notation>
    </owl:Class>
    


    <!-- http://www.cidoc-crm.org/cidoc-crm/E24_Physical_Human-Made_Thing -->

    <owl:Class rdf:about="http://www.cidoc-crm.org/cidoc-crm/E24_Physical_Human-Made_Thing">
        <rdfs:subClassOf rdf:resource="http://www.cidoc-crm.org/cidoc-crm/E18_Physical_Thing"/>
        <rdfs:subClassOf rdf:resource="http://www.cidoc-crm.org/cidoc-crm/E71_Human-Made_Thing"/>
        <rdfs:comment>This class comprises all persistent physical items of any size that are purposely created by human activity. This class comprises, besides others, Human-Made objects, such as a sword, and Human-Made features, such as rock art. For example, a “cup and ring” carving on bedrock is regarded as instance of E24 Physical Human-Made Thing.Instances of Human-Made thing may be the result of modifying pre-existing physical things, preserving larger parts or most of the original matter and structure, which poses the question if they are new or even Human-Made, the respective interventions of production made on such original material should be obvious and sufficient to regard that the product has a new, distinct identity and intended function and is human-made. Substantial continuity of the previous matter and structure in the new product can be documented by describing the production process also as an instance of E81 Transformation.Whereas interventions of conservation and repair are not regarded to produce a new Human-Made thing, the results of preparation of natural history specimens that substantially change their natural or original state should be regarded as physical Human-Made things, including the uncovering of petrified biological features from a solid piece of stone. On the other side, scribbling a museum number on a natural object should not be regarded to make it Human-Made. This notwithstanding, parts, sections, segments, or features of a physical Human-Made thing may continue to be non-Human-Made and preserved during the production process, for example natural pearls used as a part of an eardrop.</rdfs:comment>
        <rdfs:label xml:lang="en">Physical Human-Made Thing</rdfs:label>
        <skos:notation>E24</skos:notation>
    </owl:Class>
    


    <!-- http://www.cidoc-crm.org/cidoc-crm/E28_Conceptual_Object -->

    <owl:Class rdf:about="http://www.cidoc-crm.org/cidoc-crm/E28_Conceptual_Object"/>
    


    <!-- http://www.cidoc-crm.org/cidoc-crm/E2_Temporal_Entity -->

    <owl:Class rdf:about="http://www.cidoc-crm.org/cidoc-crm/E2_Temporal_Entity"/>
    


    <!-- http://www.cidoc-crm.org/cidoc-crm/E36_Visual_Item -->

    <owl:Class rdf:about="http://www.cidoc-crm.org/cidoc-crm/E36_Visual_Item">
        <rdfs:subClassOf rdf:resource="http://www.cidoc-crm.org/cidoc-crm/E73_Information_Object"/>
        <rdfs:comment>This class comprises the intellectual or conceptual aspects of recognisable marks, images and other visual works.This class does not intend to describe the idiosyncratic characteristics of an individual physical embodiment of a visual item, but the underlying prototype. For example, a mark such as the ICOM logo is generally considered to be the same logo when used on any number of publications. The size, orientation and colour may change, but the logo remains uniquely identifiable. The same is true of images that are reproduced many times. This means that visual items are independent of their physical support.The class E36 Visual Item provides a means of identifying and linking together instances of E24 Physical Human-Made Thing that carry the same visual qualities (symbols, marks or images etc.). The property P62 depicts (is depicted by) between E24 Physical Human-Made Thing and depicted subjects (E1 CRM Entity) is a shortcut of the more fully developed path from E24 Physical Human-Made Thing through P65 shows visual item (is shown by), E36 Visual Item, P138 represents (has representation) to E1CRM Entity, which in addition captures the optical features of the depiction. </rdfs:comment>
        <rdfs:label xml:lang="en">Visual Item</rdfs:label>
        <skos:notation>E36</skos:notation>
    </owl:Class>
    


    <!-- http://www.cidoc-crm.org/cidoc-crm/E39_Actor -->

    <owl:Class rdf:about="http://www.cidoc-crm.org/cidoc-crm/E39_Actor">
        <rdfs:subClassOf rdf:resource="http://www.cidoc-crm.org/cidoc-crm/E77_Persistent_Item"/>
        <rdfs:comment>This class comprises people, either individually or in groups, who have the potential to perform intentional actions of kinds for which someone may be held responsible. </rdfs:comment>
        <rdfs:label xml:lang="en">Actor</rdfs:label>
        <skos:notation>E39</skos:notation>
    </owl:Class>
    


    <!-- http://www.cidoc-crm.org/cidoc-crm/E4_Period -->

    <owl:Class rdf:about="http://www.cidoc-crm.org/cidoc-crm/E4_Period"/>
    


    <!-- http://www.cidoc-crm.org/cidoc-crm/E52_Time-Span -->

    <owl:Class rdf:about="http://www.cidoc-crm.org/cidoc-crm/E52_Time-Span">
        <rdfs:subClassOf rdf:resource="http://www.cidoc-crm.org/cidoc-crm/E1_CRM_Entity"/>
        <rdfs:comment>This class comprises abstract temporal extents, in the sense of Galilean physics, having a beginning, an end and a duration. Instances of E52 Time-Span have no semantic connotations about phenomena happening within the temporal extent they represent. They do not convey any meaning other than a positioning on the “time-line” of chronology. The actual extent of an instance of E52 Time-Span can be approximated by properties of E52 Time-Span giving inner and outer bounds in the form of dates (instances of E61 Time Primitive). Comparing knowledge about time-spans is fundamental for chronological reasoning.Some instances of E52 Time-Span may be defined as the actual, in principle observable, temporal extent of instances of E2 Temporal Entity via the property P4 has time-span (is time-span of): E52 Time-Span. They constitute phenomenal time-spans as defined in CRMgeo (Doerr   Hiebel 2013). Since our knowledge of history is imperfect and physical phenomena are fuzzy in nature, the extent of phenomenal time-spans can only be described in approximation. An extreme case of approximation, might, for example, define an instance of E52 Time-Span having unknown beginning, end and duration. It may, nevertheless, be associated with other descriptions by which we can infer knowledge about it, such as in relative chronologies.Some instances of E52 may be defined precisely as representing a declaration of a temporal extent, as, for instance, done in a business contract. They constitute declarative time-spans as defined in CRMgeo (Doerr   Hiebel 2013) and can be described via the property E61 Time Primitive P170 defines time (time is defined by): E52 Time-Span. When used as a common E52 Time-Span for two events, it will nevertheless describe them as being simultaneous, even if nothing else is known.</rdfs:comment>
        <rdfs:comment xml:lang="en">This class comprises abstract temporal extents, in the sense of Galilean physics, having a beginning, an end, and a duration.
Instances of E52 Time-Span have no semantic connotations about phenomena happening within the temporal extent they represent. They do not convey any meaning other than a positioning on the “time-line” of chronology. The actual extent of an instance of E52 Time-Span can be approximated by properties of E52 Time-Span giving inner and outer bounds in the form of dates (instances of E61 Time Primitive). Comparing knowledge about time-spans is fundamental for chronological reasoning.
Some instances of E52 Time-Span may be defined as the actual, in principle observable, temporal extent of instances of E2 Temporal Entity via the property P4 has time-span (is time-span of): E52 Time-Span. They constitute phenomenal time-spans as defined in CRMgeo (Doerr &amp;amp; Hiebel 2013). Since our knowledge of history is imperfect and physical phenomena are fuzzy in nature, the extent of phenomenal time-spans can only be described in approximation. An extreme case of approximation, might, for example, define an instance of E52 Time-Span having unknown beginning, end and duration. It may, nevertheless, be associated with other descriptions by which people can infer knowledge about it, such as in relative chronologies.
Some instances of E52 may be defined precisely as representing a declaration of a temporal extent, as, for instance, done in a business contract. They constitute declarative time-spans as defined in CRMgeo (Doerr &amp;amp; Hiebel 2013) and can be described via the property E61 Time Primitive P170 defines time (time is defined by): E52 Time-Span.
When used as a common E52 Time-Span for two events, it will nevertheless describe them as being simultaneous, even if nothing else is known.</rdfs:comment>
        <rdfs:label xml:lang="en">Time-Span</rdfs:label>
        <skos:notation>E52</skos:notation>
    </owl:Class>
    


    <!-- http://www.cidoc-crm.org/cidoc-crm/E53_Place -->

    <owl:Class rdf:about="http://www.cidoc-crm.org/cidoc-crm/E53_Place">
        <rdfs:subClassOf rdf:resource="http://www.cidoc-crm.org/cidoc-crm/E1_CRM_Entity"/>
        <rdfs:comment xml:lang="en">This class comprises extents in the natural space where people live, in particular on the surface of the Earth, in the pure sense of physics: independent from temporal phenomena and matter. They may serve describing the physical location of things or phenomena or other areas of interest. Geometrically, instances of E53 Place constitute single contiguous areas or a finite aggregation of disjoint areas in space which are each individually contiguous. They may have fuzzy boundaries.
The instances of E53 Place are usually determined by reference to the position of “immobile” objects such as buildings, cities, mountains, rivers, or dedicated geodetic marks, but may also be determined by reference to mobile objects. A Place can be determined by combining a frame of reference and a location with respect to this frame.
It is sometimes argued that instances of E53 Place are best identified by global coordinates or absolute reference systems. However, relative references are often more relevant in the context of cultural documentation and tend to be more precise. In particular, people are often interested in position in relation to large, mobile objects, such as ships. For example, the Place at which Nelson died is known with reference to a large mobile object, i.e. H.M.S Victory. A resolution of this Place in terms of absolute coordinates would require knowledge of the movements of the vessel and the precise time of death, either of which may be revised, and the result would lack historical and cultural relevance.
Any instance of E18 Physical Thing can serve as a frame of reference for an instance of E53 Place. This may be documented using the property P157 is at rest relative to (provides reference space for).</rdfs:comment>
        <rdfs:label xml:lang="en">Place</rdfs:label>
    </owl:Class>
    


    <!-- http://www.cidoc-crm.org/cidoc-crm/E55_Type -->

    <owl:Class rdf:about="http://www.cidoc-crm.org/cidoc-crm/E55_Type">
        <rdfs:subClassOf rdf:resource="http://www.cidoc-crm.org/cidoc-crm/E28_Conceptual_Object"/>
        <rdfs:comment>This class comprises concepts denoted by terms from thesauri and controlled vocabularies used to characterize and classify instances of CIDOC CRM classes. Instances of E55 Type represent concepts in contrast to instances of E41 Appellation which are used to name instances of CIDOC CRM classes. E55 Type is the CIDOC CRM’s interface to domain specific ontologies and thesauri. These can be represented in the CIDOC CRM as subclasses of E55 Type, forming hierarchies of terms, i.e., instances of E55 Type linked via P127 has broader term (has narrower term): E55 Type. Such hierarchies may be extended with additional properties. </rdfs:comment>
        <rdfs:comment xml:lang="en">This class comprises concepts denoted by terms from thesauri and controlled vocabularies used to characterize and classify instances of CIDOC CRM classes. Instances of E55 Type represent concepts, in contrast to instances of E41 Appellation which are used to name instances of CIDOC CRM classes.
E55 Type provides an interface to domain specific ontologies and thesauri. These can be represented in the CIDOC CRM as subclasses of E55 Type, forming hierarchies of terms, i.e. instances of E55 Type linked via P127 has broader term (has narrower term): E55 Type. Such hierarchies may be extended with additional properties.</rdfs:comment>
        <rdfs:label xml:lang="en">Type</rdfs:label>
        <skos:notation>E55</skos:notation>
    </owl:Class>
    


    <!-- http://www.cidoc-crm.org/cidoc-crm/E5_Event -->

    <owl:Class rdf:about="http://www.cidoc-crm.org/cidoc-crm/E5_Event">
        <rdfs:subClassOf rdf:resource="http://www.cidoc-crm.org/cidoc-crm/E4_Period"/>
        <rdfs:comment>This class comprises distinct, delimited and coherent processes and interactions of a material nature, in cultural, social or physical systems, involving and affecting instances of E77 Persistent Item in a way characteristic of the kind of process. Typical examples are meetings, births, deaths, actions of decision taking, making or inventing things, but also more complex and extended ones such as conferences, elections, building of a castle, or battles.While the continuous growth of a tree lacks the limits characteristic of an event, its germination from a seed does qualify as an event. Similarly, the blowing of the wind lacks the distinctness and limits of an event, but a hurricane, flood or earthquake would qualify as an event. Mental processes are considered as events, in cases where they are connected with the material externalization of their results; for example, the creation of a poem, a performance or a change of intention that becomes obvious from subsequent actions or declarations.The effects of an instance of E5 Event may not lead to relevant permanent changes of properties or relations of the items involved in it, for example an unrecorded performance. Of course, in order to be documented, some kind of evidence for an event must exist, be it witnesses, traces or products of the event.While instances of E4 Period always require some form of coherence between its constituent phenomena, in addition, the essential constituents of instances of E5 Event should contribute to an overall effect; for example, the statements made during a meeting and the listening of the audience.Viewed at a coarse level of detail, an instance of E5 Event may appear as if it had an ‘instantaneous’ overall effect, but any process or interaction of material nature in reality have an extent in time and space. At a fine level, instances of E5 Event may be analysed into component phenomena and phases within a space and timeframe, and as such can be seen as a period, regardless of the size of the phenomena. The reverse is not necessarily the case: not all instances of E4 Period give rise to a noteworthy overall effect and are thus not instances of E5 Event.</rdfs:comment>
        <rdfs:label xml:lang="en">Event</rdfs:label>
        <skos:notation>E5</skos:notation>
    </owl:Class>
    


    <!-- http://www.cidoc-crm.org/cidoc-crm/E63_Beginning_of_Existence -->

    <owl:Class rdf:about="http://www.cidoc-crm.org/cidoc-crm/E63_Beginning_of_Existence"/>
    


    <!-- http://www.cidoc-crm.org/cidoc-crm/E64_End_of_Existence -->

    <owl:Class rdf:about="http://www.cidoc-crm.org/cidoc-crm/E64_End_of_Existence"/>
    


    <!-- http://www.cidoc-crm.org/cidoc-crm/E71_Human-Made_Thing -->

    <owl:Class rdf:about="http://www.cidoc-crm.org/cidoc-crm/E71_Human-Made_Thing"/>
    


    <!-- http://www.cidoc-crm.org/cidoc-crm/E73_Information_Object -->

    <owl:Class rdf:about="http://www.cidoc-crm.org/cidoc-crm/E73_Information_Object"/>
    


    <!-- http://www.cidoc-crm.org/cidoc-crm/E77_Persistent_Item -->

    <owl:Class rdf:about="http://www.cidoc-crm.org/cidoc-crm/E77_Persistent_Item"/>
    


    <!-- http://www.cidoc-crm.org/cidoc-crm/E79_Part_Addition -->

    <owl:Class rdf:about="http://www.cidoc-crm.org/cidoc-crm/E79_Part_Addition">
        <rdfs:subClassOf rdf:resource="http://www.cidoc-crm.org/cidoc-crm/E11_Modification"/>
        <rdfs:comment>This class comprises activities that result in an instance of E18 Physical Thing being increased, enlarged or augmented by the addition of a part. Typical scenarios include the attachment of an accessory, the integration of a component, the addition of an element to an aggregate object, or the accessioning of an object into a curated instance of E78 Curated Holding. Both the E18 Physical Thing being augmented and the E18 Physical Thing that is being added are treated as separate identifiable wholes prior to the instance of E79 Part Addition. Following the addition of parts, the resulting assemblages are treated objectively as single identifiable wholes, made up of constituent or component parts bound together either physically (for example the engine becoming a part of the car), or by sharing a common purpose (such as the 32 chess pieces that make up a chess set). This class of activities forms a basis for reasoning about the history and continuity of identity of objects that are integrated into other objects over time, such as precious gemstones being repeatedly incorporated into different items of jewellery, or cultural artefacts being added to different museum instances of E78 Curated Holding over their lifespan..</rdfs:comment>
        <rdfs:label xml:lang="en">Part Addition</rdfs:label>
        <skos:notation>E79</skos:notation>
    </owl:Class>
    


    <!-- http://www.cidoc-crm.org/cidoc-crm/E7_Activity -->

    <owl:Class rdf:about="http://www.cidoc-crm.org/cidoc-crm/E7_Activity">
        <rdfs:subClassOf rdf:resource="http://www.cidoc-crm.org/cidoc-crm/E5_Event"/>
    </owl:Class>
    


    <!-- http://www.cidoc-crm.org/cidoc-crm/E80_Part_Removal -->

    <owl:Class rdf:about="http://www.cidoc-crm.org/cidoc-crm/E80_Part_Removal">
        <rdfs:subClassOf rdf:resource="http://www.cidoc-crm.org/cidoc-crm/E11_Modification"/>
        <rdfs:comment>This class comprises the activities that result in an instance of E18 Physical Thing being decreased by the removal of a part.Typical scenarios include the detachment of an accessory, the removal of a component or part of a composite object, or the deaccessioning of an object from a curated collection, an instance of E78 Curated Holding. If the instance of E80 Part Removal results in the total decomposition of the original object into pieces, such that the whole ceases to exist, the activity should instead be modelled as an instance of E81 Transformation, i.e., a simultaneous destruction and production. In cases where the part removed has no discernible identity prior to its removal but does have an identity subsequent to its removal, the activity should be modelled as both an instance of E80 Part Removal and E12 Production. This class of activities forms a basis for reasoning about the history, and continuity of identity over time, of objects that are removed from other objects, such as precious gemstones being extracted from different items of jewellery, or cultural artifacts being deaccessioned from different museum collections over their lifespan.</rdfs:comment>
        <rdfs:label xml:lang="en">Part Removal</rdfs:label>
        <skos:notation>E80</skos:notation>
    </owl:Class>
    


    <!-- http://www.cidoc-crm.org/cidoc-crm/E92_Spacetime_Volume -->

    <owl:Class rdf:about="http://www.cidoc-crm.org/cidoc-crm/E92_Spacetime_Volume"/>
    


    <!-- http://www.ontologydesignpatterns.org/ont/dul/DUL.owl#Collection -->

    <owl:Class rdf:about="http://www.ontologydesignpatterns.org/ont/dul/DUL.owl#Collection"/>
    


    <!-- http://www.ontologydesignpatterns.org/ont/dul/DUL.owl#Concept -->

    <owl:Class rdf:about="http://www.ontologydesignpatterns.org/ont/dul/DUL.owl#Concept">
        <owl:disjointWith rdf:resource="http://www.ontologydesignpatterns.org/ont/dul/DUL.owl#Situation"/>
    </owl:Class>
    


    <!-- http://www.ontologydesignpatterns.org/ont/dul/DUL.owl#Description -->

    <owl:Class rdf:about="http://www.ontologydesignpatterns.org/ont/dul/DUL.owl#Description">
        <owl:disjointWith rdf:resource="http://www.ontologydesignpatterns.org/ont/dul/DUL.owl#Situation"/>
        <rdfs:comment>A Description is a SocialObject that represents a conceptualization. 
It can be thought also as a &apos;descriptive context&apos; that uses or defines concepts in order to create a view on a &apos;relational context&apos; (cf. Situation) out of a set of data or observations. 
For example, a Plan is a Description of some actions to be executed by agents in a certain way, with certain parameters; a Diagnosis is a Description that provides an interpretation for a set of observed entities, etc.
Descriptions &apos;define&apos; or &apos;use&apos; concepts, and can be &apos;satisfied&apos; by situations.</rdfs:comment>
        <rdfs:isDefinedBy rdf:resource="http://www.ontologydesignpatterns.org/ont/dul/DUL.owl"/>
        <rdfs:label xml:lang="en">Description</rdfs:label>
    </owl:Class>
    


    <!-- http://www.ontologydesignpatterns.org/ont/dul/DUL.owl#Entity -->

    <owl:Class rdf:about="http://www.ontologydesignpatterns.org/ont/dul/DUL.owl#Entity"/>
    


    <!-- http://www.ontologydesignpatterns.org/ont/dul/DUL.owl#EventType -->

    <owl:Class rdf:about="http://www.ontologydesignpatterns.org/ont/dul/DUL.owl#EventType">
        <rdfs:subClassOf rdf:resource="http://www.ontologydesignpatterns.org/ont/dul/DUL.owl#Concept"/>
        <rdfs:comment>A Concept that classifies an Event . An event type describes how an Event should be interpreted, executed, expected, seen, etc., according to the Description that the EventType isDefinedIn (or used in)</rdfs:comment>
        <rdfs:comment xml:lang="en">A Concept that classifies an Event . An event type describes how an Event should be interpreted, executed, expected, seen, etc., according to the Description that the EventType isDefinedIn (or used in)</rdfs:comment>
        <rdfs:isDefinedBy rdf:resource="http://www.ontologydesignpatterns.org/ont/dul/DUL.owl"/>
        <rdfs:label xml:lang="en">Event type</rdfs:label>
    </owl:Class>
    


    <!-- http://www.ontologydesignpatterns.org/ont/dul/DUL.owl#Object -->

    <owl:Class rdf:about="http://www.ontologydesignpatterns.org/ont/dul/DUL.owl#Object">
        <rdfs:subClassOf rdf:resource="http://www.ontologydesignpatterns.org/ont/dul/DUL.owl#Entity"/>
        <rdfs:comment>Any physical, social, or mental object, or a substance. Following DOLCE Full, objects are always participating in some event (at least their own life), and are spatially located.</rdfs:comment>
        <rdfs:isDefinedBy rdf:resource="http://www.ontologydesignpatterns.org/ont/dul/DUL.owl"/>
        <rdfs:label xml:lang="en">Object</rdfs:label>
    </owl:Class>
    



    <!-- http://www.ontologydesignpatterns.org/ont/dul/DUL.owl#Situation -->

    <owl:Class rdf:about="http://www.ontologydesignpatterns.org/ont/dul/DUL.owl#Situation">
        <rdfs:subClassOf rdf:resource="http://www.ontologydesignpatterns.org/ont/dul/DUL.owl#Entity"/>
        <rdfs:comment>A view, consistent with (&apos;satisfying&apos;) a Description, on a set of entities. 
It can also be seen as a &apos;relational context&apos; created by an observer on the basis of a &apos;frame&apos; (i.e. a Description). 
For example, a PlanExecution is a context including some actions executed by agents according to certain parameters and expected tasks to be achieved from a Plan; a DiagnosedSituation is a context of observed entities that is interpreted on the basis of a Diagnosis, etc.
Situation is also able to represent reified n-ary relations, where isSettingFor is the top-level relation for all binary projections of the n-ary relation. 
If used in a transformation pattern for n-ary relations, the designer should take care of adding (some or all) OWL2 keys, corresponding to binary projections of the n-ary, to a subclass of Situation. Otherwise the &apos;identification constraint&apos; (Calvanese et al., IJCAI 2001) might be violated.</rdfs:comment>
    </owl:Class>
    


    <!-- http://www.w3.org/2006/time#Instant -->

    <owl:Class rdf:about="http://www.w3.org/2006/time#Instant">
        <rdfs:subClassOf rdf:resource="http://www.w3.org/2006/time#TemporalEntity"/>
        <owl:disjointWith rdf:resource="http://www.w3.org/2006/time#ProperInterval"/>
        <rdfs:comment xml:lang="en">A temporal entity with zero extent or duration</rdfs:comment>
        <rdfs:label xml:lang="en">Time instant</rdfs:label>
        <skos:definition xml:lang="en">A temporal entity with zero extent or duration</skos:definition>
    </owl:Class>
    


    <!-- http://www.w3.org/2006/time#Interval -->

    <owl:Class rdf:about="http://www.w3.org/2006/time#Interval">
        <rdfs:subClassOf rdf:resource="http://www.w3.org/2006/time#Interval"/>
        <rdfs:comment xml:lang="en">A temporal entity with an extent or duration</rdfs:comment>
        <rdfs:label xml:lang="en">Time interval</rdfs:label>
        <skos:definition xml:lang="en">A temporal entity with an extent or duration</skos:definition>
    </owl:Class>
    


    <!-- http://www.w3.org/2006/time#ProperInterval -->

    <owl:Class rdf:about="http://www.w3.org/2006/time#ProperInterval"/>
    


    <!-- http://www.w3.org/2006/time#TemporalEntity -->

    <owl:Class rdf:about="http://www.w3.org/2006/time#TemporalEntity">
        <owl:equivalentClass>
            <owl:Class>
                <owl:unionOf rdf:parseType="Collection">
                    <rdf:Description rdf:about="http://www.w3.org/2006/time#Instant"/>
                    <rdf:Description rdf:about="http://www.w3.org/2006/time#Interval"/>
                </owl:unionOf>
            </owl:Class>
        </owl:equivalentClass>
        <rdfs:subClassOf rdf:resource="http://www.w3.org/2002/07/owl#Thing"/>
        <rdfs:comment xml:lang="en">A temporal interval or instant.</rdfs:comment>
        <rdfs:label xml:lang="en">Temporal entity</rdfs:label>
        <skos:definition xml:lang="en">A temporal interval or instant.</skos:definition>
    </owl:Class>
    


    <!-- https://ontology.swissartresearch.net/aaao/ZE1_Institutional_Fact -->

    <owl:Class rdf:about="https://ontology.swissartresearch.net/aaao/ZE1_Institutional_Fact">
        <rdfs:subClassOf rdf:resource="http://www.cidoc-crm.org/cidoc-crm/E2_Temporal_Entity"/>
        <rdfs:comment xml:lang="en">An instance of institutional fact is an ascription of a status function to an object by a community. The institutional fact is a concretization of a collective intentionality of the community in question towards a certain object over a certain period of time.
An instance of institutional fact is recognizable to a competent speaker/member of a symbolic community (native or learner with sufficient competence). It may not be perceived through a single sense impression but through multiple experiences and implicit reasonings (e.g.: embedded participation, behavioural observation, linguistic evidence and interview), yet typically such intermediate observations and inferences are not necessarily recorded or accessible. The historical statement is typically the assertion of the institutional fact, that such and such a fact was the case, and was in force for a given community, at some time. The epistemic veridicality of the stated /reference instance of institutional fact is always open to contestation. The means of contestation involve analyzing the sources which support it.
Instances of institutional fact come into existence based on conventions establishing the conditions under which they come into effect. Typically, an instance of institutional fact will come into existence either because of the performance of its stipulated, initiating speech act (e.g.: state of being married via marriage) or as a result of events fulfilling existing norm prescriptions in the community (e.g.: state of being uncle as result of birth of child of sister).  An institutional fact comes to be through the agreed fiat of a community. It typically ceases to exist either because of a stipulated, nullifying speech act (e.g. divorce proceeding), because a community ceases to support the effective rule supporting its declaration (e.g.: ownership of people) or force majeure (e.g.: object ascribed function/status or community perceiving status is eliminated).</rdfs:comment>
        <rdfs:label xml:lang="en">Institutional Fact</rdfs:label>
        <skos:notation>ZE1</skos:notation>
    </owl:Class>
    


    <!-- https://ontology.swissartresearch.net/aaao/ZE37_Population -->

    <owl:Class rdf:about="https://ontology.swissartresearch.net/aaao/ZE37_Population"/>
    


    <!-- https://ontology.swissartresearch.net/aaao/ZE4_Classificatory_Status -->

    <owl:Class rdf:about="https://ontology.swissartresearch.net/aaao/ZE4_Classificatory_Status">
        <rdfs:subClassOf rdf:resource="https://ontology.swissartresearch.net/aaao/ZE1_Institutional_Fact"/>
        <rdfs:comment>An instance of classificatory status is the collective ascription of a type to an object by a community. The substance of the classificatory status is the communal commitment to the classification of the object in question according to the designated type.
Instances of classificatory status are recognizable through evidence of community members adopting the intentional stance of so-classifying the object in question, as observable from direct witnesses, through the reports of competent observers or through evidence of a declarative act [e.g.: E17 Type Assignment] initiating this status.
Instances of classificatory status may come to be through a formal process such as a declarative act of classification [E17 Type Assignment], or may have arisen through habit, fiat or be of unknown origin. Instances of classificatory status may end either though a formal process, such as a new declarative act of classification, be officially declassified, or may simply fade out of use, be eliminated by fiat or be of unknown reason. </rdfs:comment>
        <rdfs:comment xml:lang="en">An instance of classificatory status is the collective ascription of a type to an object by a community. The substance of the classificatory status is the communal commitment to the classification of the object in question according to the designated type.
Instances of classificatory status are recognizable through evidence of community members adopting the intentional stance of so-classifying the object in question, as observable from direct witnesses, through the reports of competent observers or through evidence of a declarative act [e.g.: E17 Type Assignment] initiating this status.
Instances of classificatory status may come to be through a formal process such as a declarative act of classification [E17 Type Assignment], or may have arisen through habit, fiat or be of unknown origin. Instances of classificatory status may end either though a formal process, such as a new declarative act of classification, be officially declassified, or may simply fade out of use, be eliminated by fiat or be of unknown reason. </rdfs:comment>
        <rdfs:label xml:lang="en">Classificatory Status</rdfs:label>
        <rdfs:label>ZE4 Classificatory Status</rdfs:label>
        <skos:notation>ZE4</skos:notation>
    </owl:Class>
    


    <!-- https://ontology.swissartresearch.net/aaao/ZE5_Function_Status -->

    <owl:Class rdf:about="https://ontology.swissartresearch.net/aaao/ZE5_Function_Status">
        <rdfs:subClassOf rdf:resource="https://ontology.swissartresearch.net/aaao/ZE4_Classificatory_Status"/>
        <rdfs:comment>An instance of function status is the collective ascription of an operative functionality to an object by a community. The substance of the function status is the communal commitment to relating to and / or using the object in question according to a designated function.
Instances of function status are recognizable through evidence of community members adopting the intentional stance of so using or relating to the object in question, as observable from direct witnesses, through the reports of competent observers or through evidence of a declarative act [e.g.: E17 Type Assignment] initiating this status.
Instances of function status may come to be through a formal process such as a declarative act of classification [E17 type Assignment], or may have arisen through habit, fiat or be of unknown origin. Instances of function status may end either though a formal process, such as a new declarative act of classification, or may simply fade out of use, be eliminated by fiat or by unknown reason.</rdfs:comment>
        <rdfs:comment xml:lang="en">An instance of function status is the collective ascription of an operative functionality to an object by a community. The substance of the function status is the communal commitment to relating to and / or using the object in question according to a designated function.
Instances of function status are recognizable through evidence of community members adopting the intentional stance of so using or relating to the object in question, as observable from direct witnesses, through the reports of competent observers or through evidence of a declarative act [e.g.: E17 Type Assignment] initiating this status.
Instances of function status may come to be through a formal process such as a declarative act of classification [E17 type Assignment], or may have arisen through habit, fiat or be of unknown origin. Instances of function status may end either though a formal process, such as a new declarative act of classification, or may simply fade out of use, be eliminated by fiat or by unknown reason.</rdfs:comment>
        <rdfs:label xml:lang="en">Function Status</rdfs:label>
        <rdfs:label xml:lang="en">ZE5 Function Status</rdfs:label>
        <skos:notation>ZE5</skos:notation>
    </owl:Class>
    


    <!-- https://w3id.org/chint/ois/ObjectInRecurrentEvent -->

    <owl:Class rdf:about="https://w3id.org/chint/ois/ObjectInRecurrentEvent"/>
    


    <!-- https://w3id.org/chint/ontology/ConceptualVariation -->

    <owl:Class rdf:about="https://w3id.org/chint/ontology/ConceptualVariation">
        <rdfs:subClassOf rdf:resource="http://www.cidoc-crm.org/cidoc-crm/E7_Activity"/>
        <rdfs:comment>The class identifies an activity that modifies immaterial visual traits of a CH object, such as the subject depicted, creating two versions of the immaterial object, which correspond to the version preceding the intervention and the one resulting from it.</rdfs:comment>
    </owl:Class>
    


    <!-- https://w3id.org/chint/ontology/Culture -->

    <owl:Class rdf:about="https://w3id.org/chint/ontology/Culture">
        <rdfs:comment xml:lang="en">Fuzzy class to indicate the broad concept of culture of which the frame observes some features (e.g., Belief that St. Servatius drunk from the drinking cup)</rdfs:comment>
        <rdfs:label xml:lang="en">Culture</rdfs:label>
    </owl:Class>
    


    <!-- https://w3id.org/chint/ontology/Function -->

    <owl:Class rdf:about="https://w3id.org/chint/ontology/Function">
        <rdfs:subClassOf rdf:resource="http://www.cidoc-crm.org/cidoc-crm/E55_Type"/>
        <rdfs:comment>A class identifying the function that an object acquires (e.g., the “drinking” function of a vessel or a liturgic function of a religious object)</rdfs:comment>
        <rdfs:label xml:lang="en">Function</rdfs:label>
    </owl:Class>
    


    <!-- https://w3id.org/chint/ontology/HistoricalFrame -->

    <owl:Class rdf:about="https://w3id.org/chint/ontology/HistoricalFrame">
        <rdfs:subClassOf rdf:resource="http://www.cidoc-crm.org/cidoc-crm/E92_Spacetime_Volume"/>
        <rdfs:comment>The Historical Frame captures the space-time continuum  to relate the observed CH object(s) to socio-cultural characteristics of the same context(s). It captures a portion of spacetime in which the CH object coexisted with immaterial, cultural traits that interacted with them.</rdfs:comment>
        <rdfs:label xml:lang="en">Historical Frame</rdfs:label>
    </owl:Class>
    


    <!-- https://w3id.org/chint/ontology/ObjectInRecurrentEvent -->

    <owl:Class rdf:about="https://w3id.org/chint/ontology/ObjectInRecurrentEvent">
        <rdfs:subClassOf rdf:resource="http://www.ontologydesignpatterns.org/ont/dul/DUL.owl#Collection"/>
        <rdfs:subClassOf rdf:resource="http://www.ontologydesignpatterns.org/ont/dul/DUL.owl#Situation"/>
        <rdfs:comment xml:lang="en">Objects observed in situations of events repeated over time, either in regular or irregular intervals, presenting unifying characteristics.</rdfs:comment>
        <rdfs:label xml:lang="en">Object in Recurrent Event</rdfs:label>
    </owl:Class>
    


    <!-- https://w3id.org/chint/ontology/ObjectInRecurrentRegularEvent -->

    <owl:Class rdf:about="https://w3id.org/chint/ontology/ObjectInRecurrentRegularEvent">
        <rdfs:subClassOf rdf:resource="https://w3id.org/chint/ontology/ObjectInRecurrentEvent"/>
        <rdfs:comment>A situation in which unifying characteristics of events regularly recurring over time are identified, and the time interval with which they are repeated can be indicated.</rdfs:comment>
        <rdfs:label xml:lang="en">Object in Recurrent Regular Event</rdfs:label>
        <rdfs:seeAlso>http://www.ontologydesignpatterns.org/cp/owl/recurrenteventseries.owl</rdfs:seeAlso>
    </owl:Class>
    


    <!-- https://w3id.org/chint/ontology/ObjectInRecurrent_IrregularEvent -->

    <owl:Class rdf:about="https://w3id.org/chint/ontology/ObjectInRecurrent_IrregularEvent">
        <rdfs:subClassOf rdf:resource="https://w3id.org/chint/ontology/ObjectInRecurrentEvent"/>
        <rdfs:comment>A situation grouping events in which the same object participates having similar, unifying characteristics over time (e.g., function).</rdfs:comment>
        <rdfs:label>Object in Recurrent Irregular Event</rdfs:label>
    </owl:Class>
    


    <!-- https://w3id.org/chint/ontology/PracticalFunction -->

    <owl:Class rdf:about="https://w3id.org/chint/ontology/PracticalFunction">
        <rdfs:subClassOf rdf:resource="https://w3id.org/chint/ontology/Function"/>
        <owl:disjointWith rdf:resource="https://w3id.org/chint/ontology/SocialFunction"/>
        <rdfs:comment xml:lang="en">A class identifying the practical function that an object acquires (e.g., the “drinking” function of a vessel)</rdfs:comment>
        <rdfs:label xml:lang="en">Practical Function</rdfs:label>
    </owl:Class>
    


    <!-- https://w3id.org/chint/ontology/SocialFunction -->

    <owl:Class rdf:about="https://w3id.org/chint/ontology/SocialFunction">
        <rdfs:subClassOf rdf:resource="https://w3id.org/chint/ontology/Function"/>
        <rdfs:comment>A class identifying the socially attributed, non strictly practical function that an object acquires (e.g., the healing function of St. Servatius cup in a catholic context)</rdfs:comment>
        <rdfs:label xml:lang="en">Social Function</rdfs:label>
    </owl:Class>
    


    <!-- https://w3id.org/icon/ontology/Attitude -->

    <owl:Class rdf:about="https://w3id.org/icon/ontology/Attitude">
        <rdfs:subClassOf rdf:resource="https://w3id.org/icon/ontology/CulturalPhenomenon"/>
        <rdfs:comment xml:lang="en">Example term taken from Panofsky&apos;s studies, can be used as a specification of a cultural phenomemon if it can be considered an Attitude</rdfs:comment>
        <rdfs:isDefinedBy rdf:resource="https://w3id.org/icon/ontology/ICONOntology"/>
        <rdfs:label xml:lang="en">Attitude</rdfs:label>
    </owl:Class>
    


    <!-- https://w3id.org/icon/ontology/Belief -->

    <owl:Class rdf:about="https://w3id.org/icon/ontology/Belief">
        <rdfs:subClassOf rdf:resource="https://w3id.org/icon/ontology/CulturalPhenomenon"/>
        <rdfs:comment xml:lang="en">Example term taken from Panofsky&apos;s studies, can be used as a specification of a cultural phenomemon if it can be considered a Belief</rdfs:comment>
        <rdfs:isDefinedBy rdf:resource="https://w3id.org/icon/ontology/ICONOntology"/>
        <rdfs:label xml:lang="en">Belief</rdfs:label>
    </owl:Class>
    


    <!-- https://w3id.org/icon/ontology/CulturalPhenomenon -->

    <owl:Class rdf:about="https://w3id.org/icon/ontology/CulturalPhenomenon">
        <rdfs:subClassOf rdf:resource="https://w3id.org/icon/ontology/IconologicalSubject"/>
        <rdfs:comment xml:lang="en">The cultural phenomenon entity expresses the cultural, social and historical aspects of which the work of art can be document. The iconographical evolution of subjects can have a cultural meaning as well. Also the personal characteristics of the artist, or of the patron, can be involved (Wittkower, Van Straten). The cultural phenomena are the object of investigation of an iconological interpretation (Van Straten, 2012, p. 12), which is considered, in the current work, a level 3 interpretation.</rdfs:comment>
        <rdfs:isDefinedBy rdf:resource="https://w3id.org/icon/ontology/ICONOntology"/>
        <rdfs:label xml:lang="en">Cultural Phenomenon</rdfs:label>
    </owl:Class>
    


    <!-- https://w3id.org/icon/ontology/CulturalValue -->

    <owl:Class rdf:about="https://w3id.org/icon/ontology/CulturalValue">
        <rdfs:subClassOf rdf:resource="https://w3id.org/icon/ontology/CulturalPhenomenon"/>
        <rdfs:comment xml:lang="en">Example term taken from Panofsky&apos;s studies, can be used as a specification of a cultural phenomemon if it can be considered a CulturalValue</rdfs:comment>
        <rdfs:isDefinedBy rdf:resource="https://w3id.org/icon/ontology/ICONOntology"/>
        <rdfs:label xml:lang="en">Cultural Value</rdfs:label>
    </owl:Class>
    


    <!-- https://w3id.org/icon/ontology/IconologicalSubject -->

    <owl:Class rdf:about="https://w3id.org/icon/ontology/IconologicalSubject"/>
    


    <!-- https://w3id.org/icon/ontology/Tendency -->

    <owl:Class rdf:about="https://w3id.org/icon/ontology/Tendency">
        <rdfs:subClassOf rdf:resource="https://w3id.org/icon/ontology/CulturalPhenomenon"/>
        <rdfs:comment xml:lang="en">Example term taken from Panofsky&apos;s studies, can be used as a specification of a cultural phenomemon if it can be considered a tendency</rdfs:comment>
        <rdfs:isDefinedBy rdf:resource="https://w3id.org/icon/ontology/ICONOntology"/>
        <rdfs:label xml:lang="en">Tendency</rdfs:label>
    </owl:Class>
    <rdf:Description>
        <owl:maxCardinality rdf:datatype="http://www.w3.org/2001/XMLSchema#nonNegativeInteger">1</owl:maxCardinality>
    </rdf:Description>
    <rdf:Description>
        <owl:cardinality rdf:datatype="http://www.w3.org/2001/XMLSchema#nonNegativeInteger">1</owl:cardinality>
    </rdf:Description>
    <rdf:Description>
        <owl:minCardinality rdf:datatype="http://www.w3.org/2001/XMLSchema#nonNegativeInteger">2</owl:minCardinality>
    </rdf:Description>
    <rdf:Description>
        <owl:minCardinality rdf:datatype="http://www.w3.org/2001/XMLSchema#nonNegativeInteger">2</owl:minCardinality>
    </rdf:Description>
    <rdf:Description>
        <owl:maxCardinality rdf:datatype="http://www.w3.org/2001/XMLSchema#nonNegativeInteger">1</owl:maxCardinality>
    </rdf:Description>
    <rdf:Description>
        <owl:minCardinality rdf:datatype="http://www.w3.org/2001/XMLSchema#nonNegativeInteger">0</owl:minCardinality>
    </rdf:Description>
    <rdf:Description>
        <owl:minCardinality rdf:datatype="http://www.w3.org/2001/XMLSchema#nonNegativeInteger">2</owl:minCardinality>
    </rdf:Description>
    


    <!-- 
    ///////////////////////////////////////////////////////////////////////////////////////
    //
    // Annotations
    //
    ///////////////////////////////////////////////////////////////////////////////////////
     -->

    <rdf:Description rdf:about="https://periodo.github.io/edtf-ontology/edtfo.ttl#hasEDTFDateTimeDescription">
        <rdfs:label xml:lang="en">has EDTF datetime description</rdfs:label>
        <skos:definition xml:lang="en">Value of an interval, expressed using EDTF</skos:definition>
        <skos:example># June 2004 to August 2006

:when a time:ProperInterval ;
  edtfo:hasEDTFDateTimeDescription &quot;2004-06/2006-08&quot;^^edtf:EDTF
  .</skos:example>
    </rdf:Description>
    <rdf:Description rdf:about="https://periodo.github.io/edtf-ontology/edtfo.ttl#inEDTFDateTime">
        <rdfs:label xml:lang="en">in EDTF datetime</rdfs:label>
        <skos:definition xml:lang="en">Position of an instant, expressed using EDTF</skos:definition>
        <skos:example># the calendar year 1985

:when a time:Instant ;
  edtfo:inEDTFDateTime &quot;1985&quot;^^edtf:EDTF
  .</skos:example>
    </rdf:Description>
</rdf:RDF>



<!-- Generated by the OWL API (version 4.5.26.2023-07-17T20:34:13Z) https://github.com/owlcs/owlapi -->

